Fixed incompleteness in the relational specification of lambda lifting and updated the proof. Some cleanup is needed

certicoq/theories/L6_PCPS/lambda_lifting_correct.v
@@ -17,7 +17,8 @@ Section Lambda_lifting_correct.
   Variable cenv : cEnv.
 
   (** The invariant that relates the original function definitions with the lifted ones *)
-  Definition Funs_inv k (rho rho' : env) (σ : var -> var) (ζ : var -> option (var * fTag * list var)) :=
+  Definition Funs_inv k (rho rho' : env) (σ : var -> var)
+             (ζ : var -> option (var * fTag * list var)) : Prop :=
     forall f f' ft' fvs vs1 vs2 j ft1  rho1 rho1' B1 f1 xs1 e1,
       ζ f = Some (f', ft', fvs) ->
       M.get f rho = Some (Vfun rho1 B1 f1) ->
@@ -25,32 +26,12 @@ Section Lambda_lifting_correct.
       find_def f1 B1 = Some (ft1, xs1, e1) ->
       Some rho1' = setlist xs1 vs1 (def_funs B1 B1 rho1 rho1) ->
       exists rho2 rho2' B2 f2 xs2 e2 vs2',
-        M.get f' rho' = Some (Vfun rho2 B2 f2) /\
+        M.get (σ f') rho' = Some (Vfun rho2 B2 f2) /\
         find_def f2 B2 = Some (ft', xs2, e2) /\
         getlist (map σ fvs) rho' = Some vs2' /\
         Some rho2' = setlist xs2 (vs2 ++ vs2') (def_funs B2 B2 rho2 rho2) /\
         (j < k -> Forall2 (preord_val pr cenv j) vs1 vs2 ->
          preord_exp pr cenv j (e1, rho1') (e2, rho2')).
-
-  (* Map from the original name to the name of the lifted function *)
-  Definition lifted_name (ζ : var -> option (var * fTag * list var)) : var -> option var :=
-    fun f => (liftM (fun x => (fst (fst x)))) (ζ f).
-
-  (* Map from the original name to the list of free vars *)
-  Definition free_vars (ζ : var -> option (var * fTag * list var)) : var -> option (list var) :=
-    fun f => (liftM (fun x => snd x)) (ζ f).
-  
-  (** The domain of ζ *)
-  Definition Funs (ζ : var -> option (var * fTag * list var)) : Ensemble var :=
-    domain (lifted_name ζ).
-  
-  (** The image of ζ on its domain - i.e. the names of the lifted functions *)
-  Definition LiftedFuns (ζ : var -> option (var * fTag * list var)) : Ensemble var :=
-    image' (lifted_name ζ) (Funs ζ).
-
-  (**  The free variables of functions in ζ, alternative definition *)
-  Definition FunsFVsLst (ζ : var -> option (var * fTag * list var)) : Ensemble (list var) :=
-    fun fvs => exists f f' ft', ζ f = Some (f', ft', fvs).
   
   (** * Lemmas about [lifted_name], [Funs], [LiftedFuns], [FunsFVs] and [FunsFVsLst] *)
 
@@ -126,32 +107,31 @@ Section Lambda_lifting_correct.
   
   Lemma Funs_inv_set k rho rho' σ ζ v1 v2 x y :
     ~ In _ (Funs ζ) x ->
-    ~ In _ (LiftedFuns ζ) y ->
+    ~ In _ (LiftedFuns ζ) x ->
     ~ In _ (FunsFVs ζ) x ->
-    ~ In _ (image σ (FunsFVs ζ)) y ->
+    ~ In _ (image σ (Union _ (FunsFVs ζ) (LiftedFuns ζ))) y ->
     Funs_inv k rho rho' σ ζ ->
     Funs_inv k (M.set x v1 rho) (M.set y v2 rho') (σ {x ~> y}) ζ.
   Proof.
-    intros Hnin1 Hnin2 Hnin3 Hnin4 Hinv f f' ft' fvs vs1 vs2 j ft1  rho1 rho1' B1 f1
+    intros Hnin1 Hnin2 Hnin4 Hnin5 Hinv f f' ft' fvs vs1 vs2 j ft1  rho1 rho1' B1 f1
            xs1 e1 Hget1 Hget2 Hlen Hdef Hset.
     assert (Heq : lifted_name ζ f = Some f')
       by (unfold lifted_name; rewrite Hget1; simpl; eauto).
     assert (Hneq : f <> x)
-      by (intros Hc; subst; eapply Hnin1; eexists; eauto).    
+      by (intros Hc; subst; eapply Hnin1; eexists; eauto).
+    assert (Hneq' : f' <> x)
+      by (intros Hc; subst; eapply Hnin2; repeat eexists; eauto).    
     rewrite M.gso in Hget2; eauto. 
     edestruct Hinv as
         [rho2 [rho2' [B2 [f2 [xs2 [e2 [vs2' [Hget' [Hdef' [Hgetl [Hset' Hpre]]]]]]]]]]]; eauto.
     do 8 eexists; repeat split; eauto.
-    - rewrite M.gso. eassumption. intros Hc; subst.
-      eapply Hnin2. eexists; split; eauto. repeat eexists; eauto.
-    - rewrite getlist_set_neq. rewrite map_extend_not_In. eassumption.
-      intros Hc. eapply Hnin3. now repeat eexists; eauto.
+    - rewrite extend_gso; eauto. rewrite M.gso; eauto.
+      intros Hc; subst.
+      eapply Hnin5. eexists; split; eauto. right. repeat eexists; eauto.
+    - rewrite map_extend_not_In. rewrite getlist_set_neq. eassumption.
       intros Hc. eapply in_map_iff in Hc. destruct Hc as [x' [Heq' HIn]].
-      destruct (peq x x') as [ Heq'' | Hneq' ].
-      eapply Hnin3. repeat eexists. eassumption. rewrite Heq''.
-      eassumption.
-      rewrite extend_gso in Heq'; eauto. eapply Hnin4.
-      repeat eexists; eassumption.
+      eapply Hnin5. eexists; split; eauto. left. now repeat eexists; eauto.
+      intros Hc. eapply Hnin4. repeat eexists. eassumption. eassumption.
   Qed.
 
   Lemma Funs_inv_setlist k rho rho' rho1 rho1' σ ζ vs1 vs2 xs ys :
@@ -159,9 +139,9 @@ Section Lambda_lifting_correct.
     setlist ys vs2 rho' = Some rho1' ->
     Funs_inv k rho rho' σ ζ ->                        
     Disjoint _ (Funs ζ) (FromList xs) ->
-    Disjoint _ (LiftedFuns ζ) (FromList ys) ->
+    Disjoint _ (LiftedFuns ζ) (FromList xs) ->
     Disjoint _ (FunsFVs ζ) (FromList xs) ->
-    Disjoint _ (image σ (Setminus _ (FunsFVs ζ) (FromList xs))) (FromList ys) ->
+    Disjoint _ (image σ (Setminus _ (Union _ (FunsFVs ζ) (LiftedFuns ζ)) (FromList xs))) (FromList ys) ->
     Funs_inv k rho1 rho1' (σ <{xs ~> ys}>) ζ.
   Proof.
     intros Hset1 Hset2 Hinv HD1 HD2 HD3 HD4 f f' ft' fvs vs1' vs2' j ft1  rho2 rho2' B1 f1
@@ -173,8 +153,12 @@ Section Lambda_lifting_correct.
     edestruct Hinv as
         [rho3 [rho3' [B2 [f2 [xs2 [e2 [vs2'' [Hget' [Hdef' [Hgetl [Hset' Hpre]]]]]]]]]]]; eauto.
     do 8 eexists; repeat split; eauto.
-    - erewrite <- setlist_not_In; eauto.
-      intros Hc; subst. eapply HD2. constructor; eauto.
+    - rewrite extend_lst_gso. erewrite <- setlist_not_In; eauto.
+      intros Hc; subst. eapply HD4. constructor; eauto.
+      eexists. split; eauto. constructor. right. now repeat eexists; eauto.
+      intros Hc'; subst. eapply HD2. constructor; eauto.
+      now repeat eexists; eauto.
+      intros Hc'; subst. eapply HD2. constructor; eauto.
       now repeat eexists; eauto.
     - erewrite getlist_setlist_Disjoint; eauto.
       rewrite map_extend_lst_Disjoint. eassumption.
@@ -185,12 +169,49 @@ Section Lambda_lifting_correct.
       intros x Hin. unfold In, FromList in Hin. eapply list_in_map_inv in Hin.
       edestruct Hin as [x' [Heq' Hin']]. eexists; split; eauto.
       constructor. 
-      repeat eexists; eassumption.
+      left. repeat eexists; eassumption.
       intros Hc. eapply HD3. constructor; eauto.
       now repeat eexists; eauto.
       eapply Disjoint_Included_l; [| eassumption ].
       repeat eexists; eassumption.
   Qed.
+
+  Lemma get_reset_lst σ xs ys (vs : list val) rho rho' z  : 
+    setlist ys vs rho = Some rho' ->
+    getlist (map σ xs) rho = Some vs ->
+    ~ In _ (FromList ys) (σ z) ->
+    length xs = length ys ->
+    NoDup xs -> NoDup ys ->
+    M.get (σ z) rho = M.get (σ <{ xs ~> ys }> z) rho'.
+  Proof with now eauto with Ensembles_DB.
+    revert σ ys vs rho' rho. induction xs as [| x xs IHxs ];
+      intros σ ys vs rho' rho Hset Hget HD Hlen Hnd1 Hnd2.
+    - destruct ys; try discriminate.
+      inv Hget. inv Hset. reflexivity.
+    - destruct ys; try discriminate. simpl in *.
+      inv Hlen. destruct vs; try discriminate.
+      destruct (setlist ys vs rho) eqn:Hset'; try discriminate.
+      destruct (M.get (σ x) rho) eqn:Hget'; try discriminate.
+      destruct (getlist (map σ xs) rho) eqn:Hgetl; try discriminate.
+      inv Hget. inv Hset. inv Hnd1. inv Hnd2. rewrite !FromList_cons in HD.
+      assert (H : M.get ((σ <{ xs ~> ys }> {x ~> e}) z) (M.set e v t) =
+                  M.get (σ <{ xs ~> ys }> z) t).
+      { destruct (peq x z); subst.
+        - rewrite extend_gss, M.gss.
+          rewrite extend_lst_gso; eauto.
+          erewrite <- setlist_not_In. symmetry. eassumption.
+          eassumption.
+          intros Hc. eapply HD. right; eauto.
+        - rewrite extend_gso; eauto. rewrite M.gso. reflexivity.
+          destruct (in_dec peq z xs).
+          + edestruct (extend_lst_gss σ) as [y' [Hin' Heq']]; eauto.
+            intros Hc. congruence.
+          + rewrite extend_lst_gso; eauto.
+            intros Hc. subst. eapply HD. constructor; eauto. }
+      rewrite H.
+      erewrite <- IHxs; eauto.
+  Qed.
+
 
   Lemma Funs_inv_setlist_getlist_r k rho rho' rho'' σ ζ vs xs ys :
     setlist ys vs rho' = Some rho'' ->
@@ -198,24 +219,23 @@ Section Lambda_lifting_correct.
     Funs_inv k rho rho' σ ζ ->
     NoDup ys -> NoDup xs ->
     length xs = length ys ->
-    Disjoint _ (LiftedFuns ζ) (FromList ys) ->
-    Disjoint _ (image σ (FunsFVs ζ)) (FromList ys) ->
+    Disjoint _ (image σ (Union _ (FunsFVs ζ) (LiftedFuns ζ))) (FromList ys) ->
     Funs_inv k rho rho'' (σ <{xs ~> ys}>) ζ.
   Proof.
-    intros Hset1 Hgetl Hinv Hnd1 Hnd2 Hlen HD1 Hinc  f f' ft' fvs vs1'
+    intros Hset1 Hgetl Hinv Hnd1 Hnd2 Hlen HD1  f f' ft' fvs vs1'
            vs2' j ft1  rho2 rho2' B1 f1 xs1 e1 Hget1 Hget2 Hlen' Hdef Hset.
     assert (Heq : lifted_name ζ f = Some f')
       by (unfold lifted_name; rewrite Hget1; simpl; eauto).
     edestruct Hinv as
         [rho3 [rho3' [B2 [f2 [xs2 [e2 [vs2'' [Hget' [Hdef' [Hgetl' [Hset' Hpre]]]]]]]]]]]; eauto.
     do 8 eexists; repeat split; eauto.
-    - erewrite <- setlist_not_In; eauto.
+    - erewrite <- get_reset_lst; eauto.
       intros Hc; subst. eapply HD1. constructor; eauto.
-      repeat eexists; eauto.
+      eexists; split; eauto. right. repeat eexists; eauto.
     - erewrite <- getlist_reset_lst; try eassumption.
       eapply Disjoint_Included_l; [| eassumption ].
       eapply image_monotonic. 
-      intros x Hin. repeat eexists; eauto.
+      intros x Hin. left. repeat eexists; eauto.
   Qed.
 
   Lemma Funs_inv_monotonic k i rho rho' σ ζ :
@@ -239,38 +259,51 @@ Section Lambda_lifting_correct.
         [rho3 [rho3' [B2 [f2 [xs2 [e2 [vs2'' [Hget' [Hdef' [Hgetl [Hset' Hpre]]]]]]]]]]]; eauto;
     do 7 eexists; repeat split; eauto.
     rewrite <- H2. eassumption.
+    rewrite <- H2. eassumption.
+    rewrite H2. eassumption.
     rewrite H2. eassumption.
   Qed.  
   
-  Lemma Funs_inv_set_lifted k rho rho' rho1 rho2 B1 B1' ζ σ v v' ft ft' xs xs' ys fvs e1 e1' vs  :
+  Lemma Funs_inv_set_lifted k rho rho' rho1 rho2 B1 B1' ζ σ v v' ft ft' xs xs' ys fvs e1 e1' vs :
+    (* B1' is the lifted version of B1, thus it satisfies the following *)
     preord_val pr cenv k (Vfun rho1 B1 v) (Vfun rho2 B1' v) ->
 
     find_def v B1 = Some (ft, xs, e1) ->
     find_def v' B1' = Some (ft', xs ++ ys, e1') ->
-    find_def v B1' = Some (ft, xs', Eapp v' ft' (xs' ++ (map σ fvs))) ->
+    find_def v B1' = Some (ft, xs', Eapp v' ft' (xs' ++ (map σ fvs))) ->  
     NoDup xs' ->
     length xs = length xs' ->
     length ys = length fvs ->
-
+    Included _ (name_in_fundefs B1) (name_in_fundefs B1') ->
+    (* the free variables have not been shadowed between the time of the function
+       definition and the application *)
     getlist (map σ fvs) rho' = Some vs ->
     getlist (map σ fvs) rho2 = Some vs ->
 
+    (* The names of the free function vars are disjoint from the original function names *)
     Disjoint _ (Union _ (FunsFVs ζ) (FromList fvs)) (bound_var_fundefs B1) ->
+    (* The names of the LiftedFuns are disjoint from the original function names *)
     Disjoint _ (LiftedFuns ζ) (bound_var_fundefs B1) ->
+    (* Τhe image of σ on the lifted functions is disjoint form the original names *)
+    Disjoint _ (image σ (LiftedFuns ζ)) (name_in_fundefs B1) ->
+    (* Τhe image of σ on the free variables is disjoint form the original and the lifted names and [xs'] *)
     Disjoint _ (image σ (Union _ (FromList fvs) (FunsFVs ζ))) (Union _ (name_in_fundefs B1') (FromList xs')) ->
+       
     Disjoint _ (FromList xs') (name_in_fundefs B1') ->
-    ~ In _ (LiftedFuns ζ) v' ->
-    
-    preord_env_P_inj pr cenv (FromList fvs) k σ rho rho' ->
+    Disjoint _ (FunsFVs ζ) (name_in_fundefs B1') ->
+    ~ In _ (LiftedFuns ζ) v' -> ~ In _ (FromList fvs) v' ->
+    ~ In _ (image σ (LiftedFuns ζ)) v' ->
+
+    (* the invariant holds for the initial environments *)
     Funs_inv k rho rho' σ ζ ->
 
     Funs_inv k (M.set v (Vfun rho1 B1 v) rho)
              (M.set v' (Vfun rho2 B1' v')
                     (M.set v (Vfun rho2 B1' v) rho'))
-             (σ {v ~> v}) (ζ {v ~> Some (v', ft', fvs)}).
-  Proof.    
-    intros Hval Hf1 Hf2 Hf3 Hnd Hlen1 Hlen2 Hgetfvs Hgetfvs1 HD1 HD2 HD3 HD4
-           Hnin Henv Hinv.
+             (σ {v ~> v} {v' ~> v'}) (ζ {v ~> Some (v', ft', fvs)}).
+  Proof.
+    intros Hval Hf1 Hf2 Hf3 Hnd Hlen1 Hlen2 Hinc Hgetfvs Hgetfvs1 HD1 HD2 HD3 HD4 HD5 HD6
+           Hnin1 Hnin2 Hnin3 Hinv.
     intros g g' t fvsg vs1 vs2 j gt1 rho3 rho4 B g1 xs1 e2 Happ Hget Hlen Hdef Hset.
     assert (Heq1 := lifted_name_eq _ _ _ _ _ Happ).
     destruct (peq g v).
@@ -281,21 +314,20 @@ Section Lambda_lifting_correct.
       erewrite <- (getlist_length_eq _ vs); [| eassumption ].
       rewrite map_length. congruence.
       do 7 eexists. repeat split; eauto.
-      + rewrite M.gss; eauto.
-      + rewrite map_extend_not_In; eauto. rewrite !getlist_set_neq; eauto. 
+      + rewrite extend_gss. rewrite M.gss; eauto.
+      + rewrite map_extend_not_In; eauto. rewrite map_extend_not_In; eauto.
+        rewrite !getlist_set_neq; eauto.
         intros Hc.
         assert (Hin : In _ (image σ (FromList fvsg)) g1).  
         { rewrite <- FromList_map_image_FromList. eassumption. }
-        eapply HD3. constructor. 
-        eapply image_monotonic; [| eassumption ].
+        eapply HD4. constructor. eapply image_monotonic; [| eassumption ].
         now eauto with Ensembles_DB.
         left. eapply fun_in_fundefs_name_in_fundefs.
         apply find_def_correct. eassumption.
         intros Hc.
         assert (Hin : In _ (image σ (FromList fvsg)) g').
         { rewrite <- FromList_map_image_FromList. eassumption. }
-        eapply HD3. constructor.
-        eapply image_monotonic; [| eassumption ].
+        eapply HD4. constructor. eapply image_monotonic; [| eassumption ]...
         now eauto with Ensembles_DB.
         left. eapply fun_in_fundefs_name_in_fundefs.
         apply find_def_correct. eassumption.
@@ -307,39 +339,39 @@ Section Lambda_lifting_correct.
         edestruct Hval as [xs2 [e2' [rho5 [Hf5 [Hset5 Hpre5]]]]]; try eassumption.
         rewrite Hf3 in Hf5; inv Hf5. specialize (Hpre5 Hlt Hall).
         intros v1 c1 Heq' Hstep.
+        specialize (Hpre5 v1 c1 Heq' Hstep).
+        edestruct Hpre5 as [v2 [c2 [Hstep' Hval']]]. inv Hstep'.        
+        erewrite <- setlist_not_In in H2; [| now eauto |].
+        rewrite def_funs_eq in H2. inv H2. rewrite Hf2 in H5; inv H5.
         edestruct (@setlist_app val) as [rho6 [Hset6 Hset6']]. eassumption.
         erewrite setlist_length_eq; now eauto.
-        specialize (Hpre5 v1 c1 Heq' Hstep).
-        edestruct Hpre5 as [v2 [c2 [Hstep' Hval']]]. inv Hstep'.
-        erewrite <- setlist_not_In in H2; [| now eauto  |].
-        rewrite def_funs_eq in H2. inv H2. rewrite Hf2 in H5; inv H5.
         assert (Heq'' : vs0 = vs2 ++ vs).
         { edestruct (@app_getlist val) as [vs1' [vs2' [Hget1 [Hget2 Heq3]]]]; subst.
           eassumption. subst.
-          erewrite getlist_setlist in Hget1; [| | now eauto ]. inv Hget1.
+          erewrite getlist_setlist in Hget1; [| now eauto | now eauto ].
+          inv Hget1. f_equal; eauto.
           erewrite getlist_setlist_Disjoint in Hget2; [| | now eauto].
           rewrite getlist_def_funs_Disjoint in Hget2.
           rewrite Hget2 in Hgetfvs1. inv Hgetfvs1. reflexivity.
           rewrite FromList_map_image_FromList.
-          eapply Disjoint_Included ;[ | | now apply HD3 ].
+          eapply Disjoint_Included ;[ | | now apply HD4 ]...
           now eauto with Ensembles_DB.
           apply image_monotonic. now eauto with Ensembles_DB.
-          eapply Disjoint_sym. eapply Disjoint_Included ;[ | | now apply HD3 ].
+          eapply Disjoint_sym. eapply Disjoint_Included ;[ | | now apply HD4 ].
           now eauto with Ensembles_DB.
           rewrite FromList_map_image_FromList.
-          apply image_monotonic. now eauto with Ensembles_DB.
-          eassumption. } 
+          apply image_monotonic. now eauto with Ensembles_DB. } 
         subst.
         rewrite Hset4' in H8. inv H8. do 2 eexists; eauto.
         eapply fun_in_fundefs_name_in_fundefs. apply find_def_correct.
         eassumption.
-        intros Hc. eapply HD4. constructor; eauto.
+        intros Hc. eapply HD5. constructor; eauto.
         eapply fun_in_fundefs_name_in_fundefs.
         apply find_def_correct. eassumption.
     - rewrite lifted_name_extend in Heq1.
       rewrite extend_gso in Happ; rewrite extend_gso in Heq1; eauto.
       subst. rewrite M.gso in Hget; eauto.
-      assert (Hnin' : ~ In _ (FromList fvsg) v).
+      assert (Hnin'' : ~ In _ (FromList fvsg) v).
       { intros Hc. eapply HD1. constructor. left; eauto. 
         repeat eexists; eauto. apply name_in_fundefs_bound_var_fundefs.
         eapply fun_in_fundefs_name_in_fundefs. apply find_def_correct.
@@ -349,31 +381,42 @@ Section Lambda_lifting_correct.
         try eassumption.
       do 7 eexists.
       split; [| split; [| split; [| split ]]]; try eassumption.
-      + rewrite !M.gso. eassumption.
-        intros Hc; subst. eapply HD2. constructor.
-        now repeat eexists; eauto.
-        apply name_in_fundefs_bound_var_fundefs.
-        eapply fun_in_fundefs_name_in_fundefs.
-        apply find_def_correct. eassumption. intros Hc. subst.
-        apply Hnin. repeat eexists; eauto.
+      + rewrite extend_gso. rewrite extend_gso. rewrite !M.gso. eassumption.
+        * intros Hc. eapply HD3. constructor.
+          eexists; split; eauto. now repeat eexists; eauto.
+          eapply fun_in_fundefs_name_in_fundefs.
+          eapply find_def_correct. eassumption.
+        * intros Hc. eapply Hnin3.
+          eexists; split; eauto. now repeat eexists; eauto.
+        * intros Hc; subst. eapply HD2. constructor.
+          now repeat eexists; eauto.
+          eapply name_in_fundefs_bound_var_fundefs. eapply fun_in_fundefs_name_in_fundefs.
+          eapply find_def_correct. eassumption.
+        * intros Hc; subst. eapply Hnin1.
+          now repeat eexists; eauto.
       + rewrite map_extend_not_In; eauto.
+        rewrite map_extend_not_In; eauto.
         rewrite !getlist_set_neq. eassumption.
-        intros Hc. 
-        assert (Hin : In _ (image σ (FromList fvsg)) v). 
-        { rewrite <- FromList_map_image_FromList. eassumption. }
-        eapply HD3. constructor.
-        eapply image_monotonic; [| eassumption ].
-        intros x Hl. repeat eexists. right. now repeat eexists; eauto.
-        left. eapply fun_in_fundefs_name_in_fundefs.
-        apply find_def_correct. eassumption.
-        intros Hc. 
-        assert (Hin : In _ (image σ (FromList fvsg)) v'). 
-        { rewrite <- FromList_map_image_FromList. eassumption. }
-        eapply HD3. constructor.
-        eapply image_monotonic; [| eassumption ].
-        intros x Hl. repeat eexists. right. now repeat eexists; eauto.
-        left. eapply fun_in_fundefs_name_in_fundefs.
-        apply find_def_correct. eassumption.
+        * intros Hc. 
+          assert (Hin : In _ (image σ (FromList fvsg)) v). 
+          { rewrite <- FromList_map_image_FromList. eassumption. }
+          eapply HD4. constructor.
+          eapply image_monotonic; [| eassumption ].
+          intros x Hl. repeat eexists. right. now repeat eexists; eauto.
+          left. eapply fun_in_fundefs_name_in_fundefs.
+          apply find_def_correct. eassumption.
+        * intros Hc. 
+          assert (Hin : In _ (image σ (FromList fvsg)) v'). 
+          { rewrite <- FromList_map_image_FromList. eassumption. }
+          eapply HD4. constructor.
+          eapply image_monotonic; [| eassumption ].
+          intros x Hl. repeat eexists. right. now repeat eexists; eauto.
+          left. eapply fun_in_fundefs_name_in_fundefs.
+          apply find_def_correct. eassumption.
+        * intros Hc. eapply HD6. constructor; eauto.
+          now repeat eexists; eauto.
+          eapply fun_in_fundefs_name_in_fundefs.
+          eapply find_def_correct. eassumption.
   Qed.
 
   (** * Lemmas about [Add_functions] *)
@@ -399,20 +442,51 @@ Section Lambda_lifting_correct.
     - inv Hin.
   Qed.
 
+
+  Lemma Setminus_Setminus_Included {A} S1 S2 S3 :
+    Decidable S3 ->
+    Included A (Setminus _ S1 (Setminus _ S2 S3))
+             (Union _ (Setminus _ S1 S2) S3).
+  Proof.
+    intros HD x H1. inv H1. destruct HD. destruct (Dec x); eauto.
+    left; constructor; eauto. intros Hc.
+    eapply H0; constructor; eauto.
+  Qed.
+    
+
   Lemma Add_functions_image_Included P B fvs σ ζ S σ' ζ' S' :
     Add_functions B fvs σ ζ S σ' ζ' S' ->
-    Included _ (image σ' P) (Union _ (image σ (Setminus _ P (name_in_fundefs B))) (name_in_fundefs B)).
+    Included _ (image σ' P)
+             (Union _ (image σ (Setminus _ P (Union _ (name_in_fundefs B) (Setminus _ S S'))))
+                                   (Union _ (name_in_fundefs B) (Setminus _ S S'))).
   Proof with now eauto with Ensembles_DB.
     intros Hadd. revert P. induction Hadd; intros P.
-    - eapply Included_trans.
-      eapply image_extend_Included'. 
+    - eapply Included_trans. now eapply image_extend_Included'.
+      eapply Union_Included.
+      eapply Included_trans. now eapply image_extend_Included'. 
       eapply Union_Included; [| now eauto with Ensembles_DB ].
       eapply Included_trans. eapply IHHadd.
-      rewrite Setminus_Union...
-    - now eauto with Ensembles_DB.
+      simpl. eapply Included_Union_compat.
+      rewrite !Setminus_Union. eapply image_monotonic.
+      eapply Included_Setminus_compat. reflexivity.
+      apply Union_Included. now eauto with Ensembles_DB.
+      eapply Included_trans. eapply Setminus_Setminus_Included.
+      now eauto with typeclass_instances.
+      now eauto with Ensembles_DB.
+      apply Union_Included. now eauto with Ensembles_DB.
+      apply Included_Union_preserv_r. apply Included_Setminus_compat.
+      reflexivity. now eauto with Ensembles_DB.
+      simpl. do 2 apply Included_Union_preserv_r.
+      apply Singleton_Included. constructor.
+      eapply Add_functions_free_set_Included; now eauto.
+      intros Hc; inv Hc; eauto.
+    - simpl. rewrite Setminus_Same_set_Empty_set at 1.
+      rewrite Setminus_Same_set_Empty_set at 1.
+      repeat rewrite Union_Empty_set_neut_r at 1.
+      rewrite Setminus_Empty_set_neut_r. reflexivity.
   Qed.
-
-  Lemma Add_functions_LiftedFuns_Included B fvs σ ζ S σ' ζ' S' :
+  
+  Lemma Add_functions_LiftedFuns_Included_r B fvs σ ζ S σ' ζ' S' :
     Add_functions B fvs σ ζ S σ' ζ' S' ->
     Included _ (LiftedFuns ζ') (Union _ (LiftedFuns ζ) (Setminus _ S S')).
   Proof with now eauto with Ensembles_DB.
@@ -429,6 +503,140 @@ Section Lambda_lifting_correct.
     - now eauto with Ensembles_DB.
   Qed.
 
+    Lemma image'_Union {A B} f S1 S2 :
+    Same_set B (image' f (Union A S1 S2))
+             (Union _ (image' f S1) (image' f S2)).
+  Proof.
+    split; intros x H.
+    - destruct H as [y [Hin Heq]].
+      inv Hin; [ left | right ]; eexists; eauto.
+    - inv H; destruct H0 as [y [Hin Heq]]; eexists; split; eauto.
+  Qed.
+
+  Lemma image'_Singleton_is_Some {A B} f x y :
+    f x = Some y ->
+    Same_set B (image' f (Singleton A x)) (Singleton B y).
+  Proof.
+    split; intros z H'.
+    - destruct H' as [w [Hin Heq ]].
+      inv Hin. rewrite Heq in H; inv H. eauto.
+    - inv H'. eexists; split; eauto.
+  Qed.
+
+  Lemma image'_extend_is_Some {B} f x y S :
+    Included B (image' (f {x ~> Some y}) S)
+             (Union _ (image' f (Setminus _ S (Singleton _ x))) (Singleton _ y)).
+  Proof.
+    intros z H'. 
+    destruct H' as [w [Hin Heq ]].
+    destruct (peq x w); subst.
+    - rewrite extend_gss in Heq. inv Heq.
+      eauto.
+    - rewrite extend_gso in Heq; eauto.
+      left. eexists; split; eauto.
+      constructor; eauto. intros Hc; inv Hc; congruence.
+  Qed.
+
+  Lemma image'_extend_is_Some_In_P {B} f x y S :
+    In _ S x ->
+    Same_set B (image' (f {x ~> Some y}) S)
+             (Union _ (image' f (Setminus _ S (Singleton _ x))) (Singleton _ y)).
+  Proof.
+    intros Hin. split.
+    - now apply image'_extend_is_Some; eauto.
+    - intros z H'. inv H'.
+      + destruct H as [w [Hin' Heq]].
+        destruct (peq x w); subst.
+        * inv Hin'. exfalso; eauto.
+        * inv Hin'. eexists; split; eauto.
+          rewrite extend_gso; eauto.
+      + inv H. eexists; split; eauto.
+        rewrite extend_gss; eauto.
+  Qed.
+  
+  Lemma image'_extend_is_Some_not_In_P {B} f x y S :
+    ~ In _ S x ->
+    Same_set B (image' (f {x ~> Some y}) S) (image' f S).
+  Proof.
+    intros Hnin. split.
+    - intros z H'. 
+      destruct H' as [w [Hin Heq ]].
+      destruct (peq x w); subst.
+      + rewrite extend_gss in Heq. inv Heq. exfalso; eauto.
+      + rewrite extend_gso in Heq; eauto.
+        eexists; split; eauto.
+    - intros z [w [Hin Heq]]. 
+      destruct (peq x w); subst.
+      + exfalso; eauto.
+      + eexists; split; eauto. rewrite extend_gso; eauto.
+  Qed.
+
+  Lemma image'_monotonic {A B} f S1 S2 :
+    Included A S1 S2 ->
+    Included B (image' f S1) (image' f S2).
+  Proof.
+    intros Hc x [y [Hin Heq]].
+    eexists; split; eauto.
+  Qed.
+
+  Lemma image'_Empty_set {A B} f:
+    Same_set B (image' f (Empty_set A)) (Empty_set B).
+  Proof.
+    split. now intros x [y [Hin Heq]]; inv Hin.
+    now eauto with Ensembles_DB.
+  Qed.
+
+  Lemma Setminus_Setminus_Same_set A S1 S2 S3 :
+    Decidable S3 ->
+    Included _ S3 S1 ->
+    Same_set A (Setminus A S1 (Setminus A S2 S3))
+             (Union A (Setminus A S1 S2) S3).
+  Proof.
+    intros Hd Hin. split.
+    now apply Setminus_Setminus_Included.
+    destruct Hd. intros x H. destruct (Dec x).
+    - constructor. now eapply Hin.
+      intros Hc; inv Hc; eauto.
+    - inv H.
+      + inv H1. constructor; eauto. intros Hc.
+        inv Hc; eauto.
+      + exfalso; eauto.
+  Qed.
+
+  Lemma image'_feq_subdomain {A B} (f1 f2 : A -> option B) S :
+    f_eq_subdomain S f1 f2 ->
+    Same_set B (image' f1 S) (image' f2 S).
+  Proof.
+    intros Heq; split; intros x [y [Hin Heq']]; eexists; split; eauto.
+    now rewrite <- Heq; eauto. now rewrite Heq; eauto.
+  Qed.
+
+  
+  Lemma Add_functions_lifted_name_Same_set B fvs σ ζ S σ' ζ' S' P :
+    unique_bindings_fundefs B ->
+    Disjoint _ P (name_in_fundefs B) ->
+    Add_functions B fvs σ ζ S σ' ζ' S' ->
+    Same_set _ (image' (lifted_name ζ') (Union _ P (name_in_fundefs B)))
+             (Union _ (image' (lifted_name ζ) P) (Setminus _ S S')).
+  Proof with now eauto with Ensembles_DB.
+    intros Hun HD Hadd. revert P HD; induction Hadd; intros P HD.
+    - inv Hun. rewrite lifted_name_extend. simpl.
+      rewrite image'_extend_is_Some_In_P.
+      rewrite !Setminus_Union_distr, Setminus_Same_set_Empty_set, Union_Empty_set_neut_l.
+      rewrite (Setminus_Disjoint (name_in_fundefs B)).
+      rewrite IHHadd, Setminus_Setminus_Same_set. 
+      rewrite Setminus_Disjoint, Union_assoc...
+      now eauto with typeclass_instances.
+      apply Singleton_Included.
+      now eapply Add_functions_free_set_Included; eauto.
+      eassumption.
+      eapply Disjoint_Included; [| | now apply HD ]...
+      eapply Disjoint_Included_l. now apply name_in_fundefs_bound_var_fundefs.
+      eapply Disjoint_Singleton_r. eassumption.
+      now eauto with Ensembles_DB.
+    - simpl. rewrite Union_Empty_set_neut_r, Setminus_Same_set_Empty_set, Union_Empty_set_neut_r...
+  Qed.
+
   Lemma Add_functions_Funs_Included B fvs σ ζ S σ' ζ' S' :
     Add_functions B fvs σ ζ S σ' ζ' S' ->
     Included _ (Funs ζ') (Union _ (Funs ζ) (name_in_fundefs B)).
@@ -441,6 +649,43 @@ Section Lambda_lifting_correct.
       now eauto with Ensembles_DB.
       eapply Included_Union_preserv_r...
     - now eauto with Ensembles_DB.
+  Qed.
+
+  Lemma domain_extend_is_Some_Same_set {A} f x (y : A) :
+    Same_set _ (domain (f {x ~> Some y})) (Union _ (domain f) (Singleton _ x)).
+  Proof. 
+    split; intros z H.
+    - destruct H as [w H'].
+      destruct (peq x z); subst; eauto.
+      rewrite extend_gso in H'; eauto. left.
+      eexists; eauto.
+    - destruct (peq x z); subst; eauto.
+      + eexists. rewrite extend_gss; eauto.
+      + inv H. destruct H0.
+        eexists. rewrite extend_gso; eauto.
+        inv H0; congruence.
+  Qed.
+
+  Lemma Add_functions_Funs_Same_set B fvs σ ζ S σ' ζ' S' :
+    Add_functions B fvs σ ζ S σ' ζ' S' ->
+    Same_set _ (Funs ζ') (Union _ (Funs ζ) (name_in_fundefs B)).
+  Proof with now eauto with Ensembles_DB.
+    intros Hadd. induction Hadd.
+    - unfold Funs. rewrite lifted_name_extend, domain_extend_is_Some_Same_set, IHHadd.
+      simpl. unfold Funs...
+    - rewrite Union_Empty_set_neut_r...
+  Qed.
+
+  Lemma Add_functions_LiftedFuns_Included_l B fvs σ ζ S σ' ζ' S' :
+    Add_functions B fvs σ ζ S σ' ζ' S' ->
+    unique_bindings_fundefs B ->
+    Disjoint _ (Funs ζ) (name_in_fundefs B) ->
+    Included _ (LiftedFuns ζ)  (LiftedFuns ζ').
+  Proof with now eauto  with Ensembles_DB.
+    intros Hadd Hun HD. unfold LiftedFuns.
+    rewrite Add_functions_Funs_Same_set with (ζ' := ζ'); eauto.
+    rewrite Add_functions_lifted_name_Same_set; eauto.
+    now eauto with Ensembles_DB.
   Qed.
 
   Lemma Add_functions_FunsFVs_Included_r B fvs σ ζ S σ' ζ' S' :
@@ -477,11 +722,16 @@ Section Lambda_lifting_correct.
 
   Lemma Add_functions_σ_eq B fvs σ ζ S σ' ζ' S' :
     Add_functions B fvs σ ζ S σ' ζ' S' ->
-    f_eq_subdomain (Complement _ (name_in_fundefs B)) σ σ'.
+    f_eq_subdomain (Complement _ (Union _ (name_in_fundefs B) (Setminus _ S S'))) σ σ'.
   Proof.
     intros Hadd. induction Hadd; simpl.
     - eapply f_eq_subdomain_extend_not_In_S_r.
-      intros Hc; apply Hc. eauto.
+      intros Hc; apply Hc.
+      eapply Singleton_Included. right. constructor.
+      eapply Add_functions_free_set_Included; eassumption.
+      intros Hc'. inv Hc'. now eauto. now eauto.
+      eapply f_eq_subdomain_extend_not_In_S_r.
+      intros Hc; apply Hc. now eauto.
       eapply f_eq_subdomain_antimon; [| eassumption ].
       now eauto with Ensembles_DB.
     - reflexivity.
@@ -503,7 +753,7 @@ Section Lambda_lifting_correct.
       destruct H1 as [x' [Hin Heq]].
       assert (Hin' : In _ (LiftedFuns ζ') f').
       now repeat eexists; eauto.
-      eapply Add_functions_LiftedFuns_Included in Hin'; [| eassumption ].
+      eapply Add_functions_LiftedFuns_Included_r in Hin'; [| eassumption ].
       inv Hin'. eapply HD.  constructor; eauto.
       eapply Add_functions_free_set_Included; eassumption.
       inv H0; eauto.
@@ -520,7 +770,7 @@ Section Lambda_lifting_correct.
 
   Lemma Add_functions_map_eq B fvs σ ζ S σ' ζ' S' l :
     Add_functions B fvs σ ζ S σ' ζ' S' ->
-    Disjoint _ (FromList l) (name_in_fundefs B) ->
+    Disjoint _ (FromList l) (Union _ (name_in_fundefs B) (Setminus _ S S'))->
     map σ l = map σ' l.
   Proof.
     intros Hadd HD. induction l; eauto.
@@ -528,9 +778,9 @@ Section Lambda_lifting_correct.
     erewrite Add_functions_σ_eq; [| eassumption |].
     rewrite IHl. reflexivity.
     now eauto with Ensembles_DB.
-    intros Hc. eapply HD; eauto.
+    intros Hc. eapply HD. constructor; eauto.
   Qed.
-
+  
   Lemma Add_functions_FunsFVs_Included_alt P B fvs σ ζ S σ' ζ' S' f f' ft fvs' :
     Add_functions B fvs σ ζ S σ' ζ' S' ->
     Disjoint _ (FunsFVs ζ) P ->
@@ -546,24 +796,24 @@ Section Lambda_lifting_correct.
       repeat eexists; eauto.
   Qed.
 
-  Lemma Add_functions_injective_subdomain P B fvs σ ζ S σ' ζ' S'  :
-    Add_functions B fvs σ ζ S σ' ζ' S' ->
-    unique_bindings_fundefs B ->
-    injective_subdomain (Setminus _ P (name_in_fundefs B)) σ ->
-    Disjoint _ (image σ (Setminus _ P (name_in_fundefs B))) (name_in_fundefs B) ->
-    injective_subdomain P σ'.
-  Proof with now eauto with Ensembles_DB.
-    intros Hadd. revert P; induction Hadd; intros P Hun Hinj HD.
-    - inv Hun. eapply injective_subdomain_extend'.
-      eapply IHHadd. eassumption. now rewrite Setminus_Union.
-      rewrite Setminus_Union...
-      intros Hc. eapply Add_functions_image_Included in Hc; [| eassumption ].
-      inv Hc. eapply HD.
-      constructor; eauto. rewrite Setminus_Union in H0; eassumption.
-      left; eauto.
-      eapply H6. eapply name_in_fundefs_bound_var_fundefs. eassumption.
-    - simpl in Hinj. now rewrite Setminus_Empty_set_neut_r in Hinj.
-  Qed.
+  (* Lemma Add_functions_injective_subdomain P B fvs σ ζ S σ' ζ' S'  : *)
+  (*   Add_functions B fvs σ ζ S σ' ζ' S' -> *)
+  (*   unique_bindings_fundefs B -> *)
+  (*   injective_subdomain (Setminus _ P (name_in_fundefs B)) σ -> *)
+  (*   Disjoint _ (image σ (Setminus _ P (name_in_fundefs B))) (name_in_fundefs B) -> *)
+  (*   injective_subdomain P σ'. *)
+  (* Proof with now eauto with Ensembles_DB. *)
+  (*   intros Hadd. revert P; induction Hadd; intros P Hun Hinj HD. *)
+  (*   - inv Hun. eapply injective_subdomain_extend'. *)
+  (*     eapply IHHadd. eassumption. now rewrite Setminus_Union. *)
+  (*     rewrite Setminus_Union... *)
+  (*     intros Hc. eapply Add_functions_image_Included in Hc; [| eassumption ]. *)
+  (*     inv Hc. eapply HD. *)
+  (*     constructor; eauto. rewrite Setminus_Union in H0; eassumption. *)
+  (*     left; eauto. *)
+  (*     eapply H6. eapply name_in_fundefs_bound_var_fundefs. eassumption. *)
+  (*   - simpl in Hinj. now rewrite Setminus_Empty_set_neut_r in Hinj. *)
+  (* Qed. *)
   
   Lemma Add_functions_image_LiftedFuns_Included B fvs σ ζ S σ' ζ' S' x f :
     Add_functions B fvs σ ζ S σ' ζ' S' ->
@@ -599,13 +849,17 @@ Section Lambda_lifting_correct.
 
   Lemma Add_functions_map_Disjoint B fvs f g S f' g' S' l :
     Add_functions B fvs f g S f' g' S' ->
-    Disjoint positive (FromList l) (name_in_fundefs B) ->
+    Disjoint positive (FromList l) (Union _ (name_in_fundefs B) (Setminus _ S S')) ->
     map f' l = map f l.
   Proof with now eauto with Ensembles_DB.
     intros Hadd HD. induction Hadd.
-    - rewrite map_extend_not_In. eapply IHHadd...
+    - rewrite !map_extend_not_In. eapply IHHadd...
       intros Hc. eapply HD; eauto.
-      constructor; eauto. left; eauto.
+      constructor; eauto. left. left; eauto.
+      intros Hc. eapply HD; eauto.
+      constructor; eauto. right. constructor; eauto.
+      eapply Add_functions_free_set_Included; eassumption.
+      intros Hc'; inv Hc'; eauto.
     - reflexivity.
   Qed.
 
@@ -732,7 +986,186 @@ Section Lambda_lifting_correct.
           now eauto with Ensembles_DB.
     - inv Hdef.
   Qed.
+
+  Lemma preord_env_P_inj_extend_not_In_P_r k P σ rho1 rho2 x y :
+    preord_env_P_inj pr cenv P k σ rho1 rho2 -> 
+    ~ In _ P x ->
+    preord_env_P_inj pr cenv P k (σ {x ~> y}) rho1 rho2.
+  Proof.
+    intros Hpre Hnin z Hp v1 Hget.
+    edestruct Hpre as [v2 [Hget2 Hpre2]]; eauto.
+    repeat eexists; eauto. rewrite extend_gso; eauto.
+    intros Hc. subst. contradiction.
+  Qed.
+
+  Lemma preord_env_P_inj_set_extend_not_In_P_r P k f rho1 rho2 x y v :
+    preord_env_P_inj pr cenv P k f rho1 rho2 ->
+    ~ In _ P x ->
+    ~ In _ (image f P) y ->
+    preord_env_P_inj pr cenv P k (f {x ~> y}) rho1 (M.set y v rho2).
+  Proof.
+    intros Henv Hnin Hnin' z Hy v' Hget.
+    edestruct Henv as [v'' [Hget' Hv]]; eauto.
+    eexists; split; eauto.
+    rewrite extend_gso, M.gso. eassumption.
+    intros Hc; subst. eapply Hnin'. now eexists; eauto.
+    intros Hc. subst. contradiction.
+  Qed.
+
+
+  Lemma lifted_name_f_eq_subdomain S f1 f2 :
+    f_eq_subdomain S f1 f2 ->
+    f_eq_subdomain S (lifted_name f1) (lifted_name f2).
+  Proof.
+    intros Heq x Hin. unfold lifted_name. simpl; rewrite Heq; eauto.
+  Qed.
+
+  Lemma Add_functions_name_in_fundefs B1 fvs σ ζ S σ' ζ' S' :
+    unique_bindings_fundefs B1 ->
+    Add_functions B1 fvs σ ζ S σ' ζ' S' ->
+    Same_set _ (image' (lifted_name ζ') (name_in_fundefs B1))
+             (Setminus var S S').
+  Proof with now eauto with Ensembles_DB.
+    intros Hun Hadd. induction Hadd; simpl in *.
+    - rewrite lifted_name_extend, image'_Union, image'_Singleton_is_Some;
+      [| now rewrite extend_gss; eauto ]. inv Hun.
+      rewrite image'_extend_is_Some_not_In_P.
+      rewrite IHHadd, Setminus_Setminus_Same_set; eauto.
+      now eauto with Ensembles_DB.
+      now eauto with typeclass_instances.
+      eapply Singleton_Included.
+      now eapply Add_functions_free_set_Included; eauto.
+      intros Hc. eapply H6.
+      now apply name_in_fundefs_bound_var_fundefs.
+    - rewrite image'_Empty_set, Setminus_Same_set_Empty_set... 
+  Qed.
+
+    
+  Lemma Fundefs_lambda_lift_name_in_fundefs_r B1 B2 σ ζ1 ζ2 S S' :
+    Fundefs_lambda_lift ζ1 σ B1 S B2 S' ->
+    unique_bindings_fundefs B1 ->
+    f_eq_subdomain (name_in_fundefs B1) ζ1 ζ2 ->
+    Same_set _ (name_in_fundefs B2)
+             (Union _ (name_in_fundefs B1) (image' (lifted_name ζ2) (name_in_fundefs B1))).
+  Proof with now eauto with Ensembles_DB.
+    intros Hfuns Hun Hfeq. induction Hfuns; simpl in *.
+    - inv Hun. rewrite IHHfuns; eauto. rewrite image'_Union.
+      rewrite !(image'_feq_subdomain (lifted_name ζ2) (lifted_name ζ)).
+      rewrite image'_Singleton_is_Some; [| erewrite lifted_name_eq; eauto ]...
+      apply lifted_name_f_eq_subdomain. symmetry.
+      eapply f_eq_subdomain_antimon; [| eassumption ]...
+      apply lifted_name_f_eq_subdomain. symmetry.
+      eapply f_eq_subdomain_antimon; [| eassumption ]...
+      eapply f_eq_subdomain_antimon; [| eassumption ]...
+    - rewrite image'_Empty_set...
+  Qed.
+
+  Lemma Add_functions_lifted_name_Disjoint_Same_set B fvs σ ζ S σ' ζ' S' P :
+    Disjoint _ P (Union _ S (name_in_fundefs B)) ->
+    Add_functions B fvs σ ζ S σ' ζ' S' ->
+    Same_set _ (image' (lifted_name ζ') P)
+             (image' (lifted_name ζ) P).
+  Proof with now eauto with Ensembles_DB.
+    intros HD Hadd. induction Hadd.
+    - rewrite lifted_name_extend. rewrite image'_extend_is_Some_not_In_P.
+      eapply IHHadd. simpl in *...
+      intros Hc. eapply HD. constructor; eauto.
+      right; left; eauto.
+    - reflexivity.
+  Qed.
+  
+  Corollary Add_functions_Fundefs_lambda_lift_name_in_fundefs
+        B1 B2 fvs σ ζ S σ1 σ2 ζ1 ζ2 S' S1 S2 :
+    Add_functions B1 fvs σ ζ S σ1 ζ1 S' ->
+    Fundefs_lambda_lift ζ2 σ2 B1 S1 B2 S2 ->
+    f_eq_subdomain (name_in_fundefs B1) ζ1 ζ2 ->
+    unique_bindings_fundefs B1 ->
+    Same_set _ (name_in_fundefs B2)
+             (Union _ (name_in_fundefs B1) (Setminus var S S')).
+  Proof.
+    intros. rewrite Fundefs_lambda_lift_name_in_fundefs_r; eauto.
+    rewrite Add_functions_name_in_fundefs; eauto. reflexivity.
+    symmetry; eauto.
+  Qed.
+
+
+  Lemma Add_functions_image_LiftedFuns_Same_set B fvs σ ζ S σ' ζ' S' :
+    Disjoint _ S (name_in_fundefs B) ->
+    unique_bindings_fundefs B ->
+    Add_functions B fvs σ ζ S σ' ζ' S' ->
+    Same_set _ (image σ' (Setminus _ S S'))
+             (Setminus _ S S').
+  Proof with now eauto with Ensembles_DB.
+    intros HD Hun Hadd. induction Hadd; simpl.
+    - inv Hun.
+      rewrite image_extend_In_S, image_extend_not_In_S, !Setminus_Setminus_Same_set,
+      !Setminus_Union_distr, Setminus_Same_set_Empty_set, Union_Empty_set_neut_r.
+      rewrite !(Setminus_Disjoint (Setminus var S S')).
+      rewrite IHHadd; eauto. reflexivity.
+      now eauto with Ensembles_DB.
+      eapply Disjoint_Singleton_r. now intros Hc; inv Hc; eauto.
+      now eauto with typeclass_instances.
+      eapply Singleton_Included.
+      now eapply Add_functions_free_set_Included; eauto.
+      intros Hc. inv Hc. inv H0.
+      eapply HD; constructor; eauto. now left; eauto.
+      constructor.
+      now eapply Add_functions_free_set_Included; eauto.
+      now intros Hc; inv Hc; eauto.
+    - rewrite !Setminus_Same_set_Empty_set, image_Empty_set...
+  Qed.
+
+  Lemma Add_functions_image_Disjoint_Same_set B fvs σ ζ S σ' ζ' S' P :
+    Disjoint _ P (Union _ S (name_in_fundefs B)) ->
+    Add_functions B fvs σ ζ S σ' ζ' S' ->
+    Same_set _ (image σ' P) (image σ P).
+  Proof with now eauto with Ensembles_DB.
+    intros HD Hadd. induction Hadd.
+    - rewrite !image_extend_not_In_S.
+      eapply IHHadd. simpl in *...
+      intros Hc; eapply HD. constructor; eauto.
+      now right; left; eauto.
+      intros Hc; eapply HD. constructor; eauto.
+      left. now eapply Add_functions_free_set_Included; eauto.
+    - reflexivity.
+  Qed.
       
+  Lemma Add_functions_image_Same_set B fvs σ ζ S σ' ζ' S' P :
+    Disjoint _ S (name_in_fundefs B) ->
+    Disjoint _ P (name_in_fundefs B) ->
+    Disjoint _ (image' (lifted_name ζ) P) (Union var S (name_in_fundefs B)) ->
+    unique_bindings_fundefs B ->
+    Add_functions B fvs σ ζ S σ' ζ' S' ->
+    Same_set _ (image σ' (image' (lifted_name ζ') (Union _ P (name_in_fundefs B))))
+             (Union _ (Setminus _ S S') (image σ (image' (lifted_name ζ) P))).
+  Proof with now eauto with Ensembles_DB.
+    intros. rewrite Add_functions_lifted_name_Same_set; eauto.
+    rewrite image_Union, Union_commut. apply Same_set_Union_compat.
+    rewrite Add_functions_image_LiftedFuns_Same_set...
+    rewrite Add_functions_image_Disjoint_Same_set; eauto.
+    reflexivity.  
+  Qed.
+
+  Lemma Add_functions_same_name B fvs σ ζ S σ' ζ' S' f :
+    In _ (Union _ (name_in_fundefs B) (Setminus _ S S')) f ->
+    Add_functions B fvs σ ζ S σ' ζ' S' ->
+    σ' f = f.
+  Proof.
+    intros Hin Hadd. induction Hadd; eauto.
+    - destruct (peq f f'); subst.
+      + rewrite extend_gss; eauto.
+      + rewrite extend_gso; eauto. destruct (peq f0 f); subst.
+        * rewrite extend_gss; eauto.
+        * rewrite extend_gso; eauto. eapply IHHadd.
+          inv Hin. inv H0. inv H1; congruence. now eauto.
+          right. inv H0. constructor; eauto.
+          intros Hc. eapply H2. constructor; eauto.
+          intros Hc'; inv Hc'; congruence.
+    - inv Hin. inv H. rewrite Setminus_Same_set_Empty_set in H. inv H.
+  Qed.
+    
+
+
   Lemma Fundefs_lambda_lift_correct k rho rho' B1 B1' B2 B2' σ ζ σ1 ζ1 σ2 ζ2 S
         S1' S1'' S1''' S2' S2'' S2''' fvs e:
     (* The IH for expressions *)
@@ -743,15 +1176,15 @@ Section Lambda_lifting_correct.
           (σ : var -> var) (S : Ensemble var) (e' : exp) 
           (S' : Ensemble var),
         unique_bindings e ->
-        Disjoint var (image σ (Union _ (occurs_free e) (FunsFVs ζ)))
-                 (Union var S (Union _ (bound_var e) (LiftedFuns ζ))) ->
+        Disjoint var (image σ (Union _ (Union _ (occurs_free e) (FunsFVs ζ)) (LiftedFuns ζ)))
+                 (Union var S (bound_var e)) ->
         Disjoint var S (Union var (bound_var e) (occurs_free e)) ->
         Disjoint var (LiftedFuns ζ) (Union _ S (bound_var e)) ->
-        Disjoint var (Funs ζ) (bound_var e) ->
-        Disjoint var (FunsFVs ζ) (bound_var e) ->
+        Disjoint var (Funs ζ) (Union _ S (bound_var e)) ->
+        Disjoint var (FunsFVs ζ) (Union _ S (bound_var e)) ->
         Disjoint _ (bound_var e) (occurs_free e) ->
-        binding_in_map (Union _ (occurs_free e) (FunsFVs ζ)) rho ->
-        preord_env_P_inj pr cenv (Union _ (occurs_free e) (FunsFVs ζ)) m σ rho rho' ->
+        binding_in_map (image σ (Union _ (Union _ (occurs_free e) (FunsFVs ζ)) (LiftedFuns ζ))) rho' ->
+        preord_env_P_inj pr cenv (occurs_free e) m σ rho rho' ->
         Funs_inv m rho rho' σ ζ ->
         Exp_lambda_lift ζ σ e S e' S' ->
         preord_exp pr cenv m (e, rho) (e', rho')) ->
@@ -761,13 +1194,13 @@ Section Lambda_lifting_correct.
      unique_bindings_fundefs B2 ->
 
      (* The image of σ is neither in the free set nor in the set of bound variables *)
-     Disjoint var (image σ (Union _ (occurs_free (Efun B1 e)) (FunsFVs ζ)))
-              (Union var S (Union _ (bound_var_fundefs B1) (LiftedFuns ζ))) ->
-     Disjoint var (image σ (Union _ (occurs_free (Efun B1 e)) (FunsFVs ζ)))
-              (Union var S (Union _ (bound_var_fundefs B2) (LiftedFuns ζ))) ->
+     Disjoint var (image σ (Union _ (occurs_free (Efun B1 e)) (Union _ (FunsFVs ζ) (LiftedFuns ζ))))
+              (Union var S (bound_var_fundefs B1)) ->
+     Disjoint var (image σ (Union _ (occurs_free (Efun B1 e)) (Union _ (FunsFVs ζ) (LiftedFuns ζ))))
+              (Union var S (bound_var_fundefs B2)) ->
 
      (* The free set is disjoint from the set of bound and free variables *)
-     Disjoint var S (Union var (bound_var_fundefs B1) (occurs_free_fundefs B1)) ->
+     Disjoint var S (Union var (bound_var_fundefs B1) (occurs_free (Efun B1 e))) ->
      Disjoint var S (Union var (bound_var_fundefs B2) (occurs_free_fundefs B2)) ->
 
      (* The names of lifted functions is neither in the free set nor in the set of bound variables*) 
@@ -775,29 +1208,31 @@ Section Lambda_lifting_correct.
      Disjoint var (LiftedFuns ζ) (Union _ S (bound_var_fundefs B2)) ->
 
      (* The domain of ζ is disjoint with the bound variables *)
-     Disjoint var (Funs ζ) (bound_var_fundefs B1) ->
+     Disjoint var (Funs ζ) (Union _ S (bound_var_fundefs B1)) ->
+     Disjoint var (Funs ζ) (Union _ S (bound_var_fundefs B2)) ->          
 
      (* The free variables of the funs in ζ are disjoint from the bound variables *) 
-     Disjoint var (FunsFVs ζ) (bound_var_fundefs B1) ->
-     Disjoint var (FunsFVs ζ) (bound_var_fundefs B2) ->
+     Disjoint var (FunsFVs ζ) (Union _ S (bound_var_fundefs B1)) ->
+     Disjoint var (FunsFVs ζ) (Union _ S (bound_var_fundefs B2)) ->
 
      (* The bound variables and the free variables are disjoint *)
      Disjoint _ (bound_var_fundefs B1) (occurs_free_fundefs B1) ->
 
      (* The free variables are in the environment *)
-     binding_in_map (Union _ (occurs_free (Efun B1 e)) (FunsFVs ζ)) rho ->
+     binding_in_map (image σ (Union _ (occurs_free (Efun B1 e)) (Union _ (FunsFVs ζ) (LiftedFuns ζ))))
+                    rho' ->
 
      (** ζ1 and ζ2 are equal in a [name_in_fundefs B2] *) 
      f_eq_subdomain (name_in_fundefs B2) ζ1 ζ2 ->
 
      (** The invariant hold for the initial environments **)
-     preord_env_P_inj pr cenv (Union _ (occurs_free (Efun B1 e)) (FunsFVs ζ)) k σ rho rho' ->
+     preord_env_P_inj pr cenv (occurs_free (Efun B1 e)) k σ rho rho' ->
      Funs_inv k rho rho' σ ζ ->
      
      NoDup fvs ->
-     Included _ (FromList fvs) (Union _ (occurs_free_fundefs B1) (FunsFVs ζ)) ->
-     Disjoint var (FromList fvs) (bound_var_fundefs B1) ->
-     Disjoint var (FromList fvs) (bound_var_fundefs B2) ->
+     Included _ (FromList fvs) (Union _ (occurs_free_fundefs B1) (Union _ (LiftedFuns ζ) (FunsFVs ζ))) ->
+     Disjoint var (FromList fvs) (Union _ S (bound_var_fundefs B1)) ->
+     Disjoint var (FromList fvs) (Union _ S (bound_var_fundefs B2)) ->
 
      Included _ (name_in_fundefs B2) (name_in_fundefs B1) ->
      
@@ -810,7 +1245,7 @@ Section Lambda_lifting_correct.
      Fundefs_lambda_lift ζ1 σ1 B2 S2'' B2' S2''' ->
 
      (** The invariants hold for the final environments **)
-     preord_env_P_inj pr cenv (Union _ (Union _ (occurs_free (Efun B1 e)) (name_in_fundefs B2)) (FunsFVs ζ1))
+     preord_env_P_inj pr cenv (Union _ (occurs_free (Efun B1 e)) (name_in_fundefs B2))
                       k σ2 (def_funs B1 B2 rho rho) (def_funs B1' B2' rho' rho') /\
      Funs_inv k (def_funs B1 B2 rho rho) (def_funs B1' B2' rho' rho') σ2 ζ2.
   Proof with now eauto with Ensembles_DB.
@@ -818,29 +1253,25 @@ Section Lambda_lifting_correct.
     induction k as [ k IH' ] using lt_wf_rec1.
     induction B2;
       intros rho rho' B1 B1' B2' σ ζ σ1 ζ1 σ2 ζ2 S S1' S1'' S1''' S2' S2'' S2''' fvs
-             IHe Hun1 Hun2 Him1 Him2 Hf1 Hf2 Hlf1 Hlf2 Hfun1 Hfvs1 Hfvs2
+             IHe Hun1 Hun2 Him1 Him2 Hf1 Hf2 Hlf1 Hlf2 Hfun1 Hfun2 Hfvs1 Hfvs2
              HD Hbin Hfeq Henv Hinv Hnd Hin HD1 HD2 Hinc Hadd1 Hinc1 Hll1 Hadd2 Hinc2 Hll2.
     - inv Hadd2. inv Hll2. inv Hun2. simpl.
       assert
         (HB1 : forall j, j < k ->
-                    preord_env_P_inj pr cenv
-                                     (Union var
-                                            (Union var (occurs_free (Efun B1 e)) (name_in_fundefs B1))
-                                            (FunsFVs ζ1)) j σ1
-                                     (def_funs B1 B1 rho rho) (def_funs B1' B1' rho' rho') /\
+                    preord_env_P_inj pr cenv (Union var (occurs_free (Efun B1 e)) (name_in_fundefs B1))
+                                     j σ1 (def_funs B1 B1 rho rho) (def_funs B1' B1' rho' rho') /\
                     Funs_inv j (def_funs B1 B1 rho rho) (def_funs B1' B1' rho' rho') σ1 ζ1).
       { intros j leq. eapply IH'; (try now apply Hll1); (try now apply Hnd);
                       (try now apply Hadd1); try eassumption.
         - intros. eapply IHe; eauto. omega.
+        - eapply Disjoint_Included; [| | now apply Hf1 ].
+          normalize_occurs_free... reflexivity.
         - reflexivity.
         - eapply preord_env_P_inj_monotonic; [| eassumption]. omega.
         - eapply Funs_inv_monotonic. eassumption. omega.
         - reflexivity. } clear IH'.
-      assert (HB2 : preord_env_P_inj pr cenv
-                                     (Union var
-                                            (Union var (occurs_free (Efun B1 e)) (name_in_fundefs B2))
-                                            (FunsFVs ζ1)) k σ'
-                                     (def_funs B1 B2 rho rho) (def_funs B1' B' rho' rho') /\
+      assert (HB2 : preord_env_P_inj pr cenv (Union var (occurs_free (Efun B1 e)) (name_in_fundefs B2))
+                                     k σ' (def_funs B1 B2 rho rho) (def_funs B1' B' rho' rho') /\
                     Funs_inv k (def_funs B1 B2 rho rho)
                              (def_funs B1' B' rho' rho') σ' ζ').
       { eapply IHB2; try (now apply Hnd);  try eassumption;
@@ -863,15 +1294,17 @@ Section Lambda_lifting_correct.
           as (xs2 & ys' & e2 & S3 & S2 & Hfind1 & Hfind2 & Hnd1
                   & Hnd2 & Hlen1 & Hlen2 & Hinc1' & Hinc2' & Hinc3' & HD1' & HD2' & HD3' & Hll).
         eassumption. eassumption.
-        eapply Disjoint_Included_r_sym. eapply Add_functions_LiftedFuns_Included. eassumption.
+        eapply Disjoint_Included_r_sym. eapply Add_functions_LiftedFuns_Included_r. eassumption.
         eapply Union_Disjoint_l. eapply Disjoint_Included_r; [| now apply Hlf1 ]...
         eapply Disjoint_Included; [| | now apply Hf1]...
         eapply Add_functions_injective_subdomain_LiftedFuns; eassumption. eassumption.
         (* Various useful assertions *)
+
         assert (Hfree : Included _ (occurs_free e1)
                                  (Union var (FromList xs1)
                                         (Union var (name_in_fundefs B1) (occurs_free_fundefs B1)))).
         { eapply occurs_free_in_fun. apply find_def_correct. eassumption. }
+
         assert (Hbound : In _ (bound_var_fundefs B1) v /\
                          Included _ (FromList xs1) (bound_var_fundefs B1) /\
                          Included _ (bound_var e1) (bound_var_fundefs B1) ).
@@ -881,49 +1314,48 @@ Section Lambda_lifting_correct.
         destruct Hbound as [Hb1 [Hb2 Hb3]].
         edestruct unique_bindings_fun_in_fundefs as [Hune1 [HunB1 [HunB2 [HunB3 [HunB4 [HunB5 HunB6]]]]]].
         exact (find_def_correct _ _ _ _ _ Hf). eassumption.
-        assert (Heq : fvs0 = fvs). 
+
+        assert (Heq : fvs0 = fvs).
         { eapply Add_functions_fvs_eq; [| eassumption |]; try eassumption.
           eapply fun_in_fundefs_name_in_fundefs. now eapply find_def_correct; eauto. }
         edestruct setlist_length2 as [rho2' Hs']; [| eassumption | now eauto | ]. eauto.
-        assert (HDim : Disjoint _ (image σ1
-                                         (Union _
-                                                (Union _ (occurs_free (Efun B1 e)) (FunsFVs ζ1))
-                                                (name_in_fundefs B1)))
-                                (Union _ S (Union _ (Union _ (bound_var e1) (FromList xs1))
-                                                  (LiftedFuns ζ1)))).
-        { eapply Disjoint_Included_l.
-          eapply Add_functions_image_Included. eassumption.
-          eapply Union_Disjoint_l.
-          eapply Disjoint_Included; [| | now apply Him1 ].
-          apply Union_Included. now eauto with Ensembles_DB.
-          apply Union_Included. now eauto with Ensembles_DB.
-          eapply Included_trans. eapply Add_functions_LiftedFuns_Included.
-          eassumption. now eauto with Ensembles_DB.
-          apply image_monotonic. apply Setminus_Included_Included_Union.
-          apply Included_Union_compat ; [| reflexivity ].
-          apply Union_Included. now eauto with Ensembles_DB.
-          eapply Included_trans. eapply Add_functions_FunsFVs_Included_r.
-          eassumption.
-          eapply Included_trans. eapply Included_Union_compat. reflexivity.
-          eassumption. normalize_occurs_free...
-          eapply Union_Disjoint_r.
-          eapply Disjoint_Included_l_sym; [| now apply Hf1 ].
-          eapply Included_Union_preserv_l. now apply name_in_fundefs_bound_var_fundefs.
-          apply Union_Disjoint_r. eapply Disjoint_sym...
-          eapply Disjoint_Included_l. now apply name_in_fundefs_bound_var_fundefs.          
-          eapply Disjoint_Included_r.  eapply Add_functions_LiftedFuns_Included.
-          eassumption. clear Hlf2 Hf2. now eauto with Ensembles_DB. }
+
         assert (Hsub : Included _ S1'' S).
         { eapply Included_trans. eassumption.
           eapply Add_functions_free_set_Included. eassumption. }
+
         assert (Hsub' : Included _ S3 S).
         { eapply Included_trans. eassumption. eassumption. }
+
+        assert (HDlfuns : Disjoint _ (LiftedFuns ζ1)
+                                   (Union _ (Union _ S1'' (Union _ (bound_var e1) (FromList xs1)))
+                                          (name_in_fundefs B1))).
+        { eapply Disjoint_Included_l. 
+          eapply Add_functions_LiftedFuns_Included_r. eassumption.
+          eapply Union_Disjoint_l.
+          eapply Disjoint_Included_r; [| now apply Hlf1 ].
+          rewrite <- Union_assoc. apply Included_Union_compat. eassumption.
+          apply Union_Included.
+          now eauto with Ensembles_DB. now apply name_in_fundefs_bound_var_fundefs.
+          eapply Union_Disjoint_r. eapply Union_Disjoint_r. 
+          eapply Disjoint_Included_r. now apply Hinc1.
+          now eauto with Ensembles_DB.
+          eapply Disjoint_Included_l. now apply Setminus_Included.
+          eapply Disjoint_Included_r; [ | now apply Hf1 ].
+          now eauto with Ensembles_DB.
+          eapply Disjoint_Included_r. now apply name_in_fundefs_bound_var_fundefs.
+          eapply Disjoint_Included_l. now apply Setminus_Included.
+          eapply Disjoint_Included_r; [ | now apply Hf1 ].
+          now eauto with Ensembles_DB. }
+        
         assert (HD' : Disjoint var (Union var (FromList xs1) (FromList ys'))
-                               (Union _ (Union var S3 (bound_var e1)) (LiftedFuns ζ1))).
+                               (Union _ (Union _ (Union var S3 (bound_var e1)) (LiftedFuns ζ1))
+                                      (name_in_fundefs B1))).
         { eapply Disjoint_Included_r. eapply Included_Union_compat.
+          eapply Included_Union_compat. reflexivity.
+          eapply Add_functions_LiftedFuns_Included_r. eassumption.
           reflexivity.
-          eapply Add_functions_LiftedFuns_Included. eassumption.
-          eapply Union_Disjoint_r. eapply Union_Disjoint_r.
+          eapply Union_Disjoint_r. eapply Union_Disjoint_r. eapply Union_Disjoint_r.
           eapply Union_Disjoint_l. eapply Disjoint_sym.
           eapply Disjoint_Included ; [ | | now apply Hf1 ].
           apply Included_Union_preserv_l; eassumption. eassumption.
@@ -941,29 +1373,56 @@ Section Lambda_lifting_correct.
           eapply Disjoint_Included ; [ | | now apply Hf1 ].
           apply Included_Union_preserv_l; eassumption. now eauto with Ensembles_DB.
           eapply Disjoint_Included_l. eapply Included_trans.
-          eassumption. now apply Hinc1. now eauto with Ensembles_DB. }
-        assert (HDfuns : Disjoint _ (Funs ζ1) (Union _ (bound_var e1) (FromList xs1))).
+          eassumption. now apply Hinc1. now eauto with Ensembles_DB.
+          eapply Union_Disjoint_l. eassumption.
+          eapply Disjoint_Included ; [ | | now apply Hf1 ].
+          apply Included_Union_preserv_l. now apply name_in_fundefs_bound_var_fundefs.
+          eapply Included_trans; eassumption. }
+
+        assert (HDim : Disjoint _ (image σ1
+                                         (Union _
+                                                (Union _ (occurs_free (Efun B1 e))
+                                                       (Union _ (LiftedFuns ζ1) (FunsFVs ζ1)))
+                                                (name_in_fundefs B1)))
+                                (Union _ S1'' (Union _ (bound_var e1) (FromList xs1)))).
+        { eapply Disjoint_Included_l. eapply Add_functions_image_Included.
+          eassumption. eapply Union_Disjoint_l.
+          eapply Disjoint_Included; [| | now apply Him1 ].
+          now eauto with Ensembles_DB.
+          apply image_monotonic. apply Setminus_Included_Included_Union.
+          apply Union_Included. apply Union_Included. now eauto with Ensembles_DB.
+          apply Union_Included. eapply Included_trans.
+          eapply Add_functions_LiftedFuns_Included_r. eassumption.
+          now eauto with Ensembles_DB.
+          eapply Included_trans.
+          eapply Add_functions_FunsFVs_Included_r. eassumption.
+          apply Union_Included. now eauto with Ensembles_DB.
+          eapply Included_trans. eassumption.
+          normalize_occurs_free... now eauto with Ensembles_DB.
+          eapply Union_Disjoint_l. eapply Disjoint_sym.
+          eapply Union_Disjoint_l; [ | eapply Union_Disjoint_l]; try eassumption.
+          eapply Disjoint_Included; [| | now apply Hf1].
+          eapply Included_Union_preserv_l. now apply name_in_fundefs_bound_var_fundefs.
+          eassumption.
+          eapply Union_Disjoint_r. eapply Disjoint_Included_r. eapply Hinc1.
+          now eauto with Ensembles_DB.
+          eapply Disjoint_Included_l. now apply Setminus_Included.
+          clear Hf2. eapply Union_Disjoint_r... }
+
+        assert (HDfuns : Disjoint _ (Funs ζ1) (Union _ S (Union _ (bound_var e1) (FromList xs1)))).
         { eapply Disjoint_Included_l.
           eapply Add_functions_Funs_Included. eassumption.
           eapply Union_Disjoint_l.
           eapply Disjoint_Included_r; [| now apply Hfun1 ].
           now eauto with Ensembles_DB.
-          eapply Union_Disjoint_r; apply Disjoint_sym; eassumption. }
-        assert (HDlfuns : Disjoint _ (LiftedFuns ζ1)
-                                   (Union _ S1'' (Union _ (bound_var e1) (FromList xs1)))).
-        { eapply Disjoint_Included_l. 
-          eapply Add_functions_LiftedFuns_Included. eassumption.
-          eapply Union_Disjoint_l.
-          eapply Disjoint_Included_r; [| now apply Hlf1 ].
-          apply Included_Union_compat. eassumption.
-          now eauto with Ensembles_DB.
           eapply Union_Disjoint_r. 
-          eapply Disjoint_Included_r. now apply Hinc1.
-          now eauto with Ensembles_DB.
-          eapply Disjoint_Included_l. now apply Setminus_Included.
-          eapply Disjoint_Included_r; [ | now apply Hf1 ].
-          now eauto with Ensembles_DB. }
-        assert (HDfunsfvs : Disjoint _ (FunsFVs ζ1) (Union _ (bound_var e1) (FromList xs1))).
+          apply Disjoint_sym. eapply Disjoint_Included_r.
+          now apply name_in_fundefs_bound_var_fundefs.
+          clear Hf2. now eauto with Ensembles_DB.
+          eapply Union_Disjoint_r; eapply Disjoint_sym; eassumption. }
+
+        assert (HDfunsfvs : Disjoint _ (FunsFVs ζ1)
+                                     (Union _ S (Union _ (bound_var e1) (FromList xs1)))).
         { eapply Disjoint_Included_l.
           eapply Add_functions_FunsFVs_Included_r. eassumption.
           eapply Union_Disjoint_l.
@@ -971,6 +1430,7 @@ Section Lambda_lifting_correct.
           now eauto with Ensembles_DB. clear HD2.
           now eauto with Ensembles_DB. }
         (* Various useful assertions end *)
+
         do 3 eexists. split. eassumption.
         split. now eauto. 
         intros Hleq Hall. intros v1 c1 Hleq' Hstep.
@@ -980,9 +1440,14 @@ Section Lambda_lifting_correct.
         eassumption. rewrite def_funs_eq. reflexivity.
         eapply fun_in_fundefs_name_in_fundefs. eapply find_def_correct.
         eassumption. eassumption. eassumption. eassumption.
+        assert (σ1 f'0 = f'0).
+        { assert (Hin' := fun_in_fundefs_name_in_fundefs _ _ _ _ _ (find_def_correct _ _ _ _ _ Hfind2)).
+          eapply Add_functions_Fundefs_lambda_lift_name_in_fundefs in Hin'; [ | | now eauto | | ]; eauto.
+          eapply Add_functions_same_name; eauto. reflexivity.
+        } rewrite H in Hget3. 
         rewrite def_funs_eq in Hget3;
-          [| eapply fun_in_fundefs_name_in_fundefs; eapply find_def_correct; eassumption ].
-        inv Hget3. rewrite Hfind3 in Hfind2. inv Hfind2.
+        [| eapply fun_in_fundefs_name_in_fundefs; eapply find_def_correct; eassumption ].
+        inv Hget3. rewrite Hfind3 in Hfind2. clear H. inv Hfind2.        
         symmetry in Hset3. edestruct (@setlist_app val) as [rho3'' [Hset1 Hset2]].
         eassumption. rewrite <- Hlen. now eapply setlist_length_eq; eauto.
         { edestruct IHe with (rho := rho1') (rho' := rho3') (e := e1) (e' := e2)
@@ -996,53 +1461,64 @@ Section Lambda_lifting_correct.
                 now eauto with Ensembles_DB.
                 eapply image_monotonic. normalize_occurs_free.
                 apply Setminus_Included_Included_Union.
-                eapply Included_trans.
-                apply Included_Union_compat. eassumption. reflexivity.
-                rewrite FromList_app. now eauto 10 with Ensembles_DB.
+                eapply Included_trans. 
+                apply Included_Union_compat. apply Included_Union_compat.
+                eassumption. reflexivity. reflexivity.
+                rewrite FromList_app. now eauto 15 with Ensembles_DB.
               * rewrite FromList_app. now eauto with Ensembles_DB.
           - (*  Disjoint _ S3 (Union _ (bound_var e1) (occurs_free e1)) *)
             eapply Disjoint_Included_l. eassumption.
             eapply Disjoint_Included_r; [| now apply Hf1 ].
+            normalize_occurs_free. rewrite Union_assoc. eapply Included_Union_preserv_l.
             eapply bound_var_occurs_free_in_fun_Included.
             apply find_def_correct. eassumption.
           - (*  Disjoint var (LiftedFuns ζ1') (bound_var  e1) *)
             now eauto with Ensembles_DB.
           - (* Disjoint var (Funs ζ1') (bound_var e1) *)
-            now eauto with Ensembles_DB.
+            clear Hfun2. now eauto with Ensembles_DB.
           - (* Disjoint var (FunsFVs ζ1') (bound_var e1) *)
+            eapply Disjoint_Included_r; [| eassumption ].
             now eauto with Ensembles_DB.
           - eapply fun_in_fundefs_Disjoint_bound_Var_occurs_free;
              [| | eassumption ]; eauto.
             eapply find_def_correct. eassumption.
-          - eapply binding_in_map_antimon.
-            eapply Included_Union_compat. eassumption.
-            eapply Add_functions_FunsFVs_Included_r. eassumption.
-            intros x Hx. rewrite <- !Union_assoc in Hx.
-            eapply binding_in_map_setlist; [| now eauto | ].
-            eapply binding_in_map_def_funs. eassumption.
-            normalize_occurs_free. inv Hx; eauto.
-            inv H; eauto. inv H0; eauto. inv H; eauto.
-            eapply Hin in H0; eauto. inv H0; eauto.
+          - eapply binding_in_map_antimon;
+            [ | eapply binding_in_map_setlist;
+                [ eapply binding_in_map_setlist;
+                  [ eapply binding_in_map_def_funs; eassumption |  eassumption ] | eassumption ]].
+            eapply Included_trans. eapply image_extend_lst_Included.
+            rewrite !app_length. congruence.
+            rewrite !FromList_app.
+            apply Union_Included; [| now eauto with Ensembles_DB ]. 
+            eapply Included_trans. eapply Add_functions_image_Included. eassumption.
+            eapply Union_Included.
+            + do 3 eapply Included_Union_preserv_r.
+              eapply image_monotonic. do 2 apply Setminus_Included_Included_Union.
+              eapply Included_trans. eapply Included_Union_compat.
+              eapply Included_Union_compat. eassumption.
+              eapply Add_functions_FunsFVs_Included_r; eauto.
+              eapply Add_functions_LiftedFuns_Included_r; eauto.
+              normalize_occurs_free. now eauto 20 with Ensembles_DB.
+            + do 2 eapply Included_Union_preserv_r.
+              eapply Included_Union_preserv_l.
+              rewrite (Add_functions_Fundefs_lambda_lift_name_in_fundefs B1 B3); eauto.
+              reflexivity. reflexivity.
           - (* preord_env_P_inj pr cenv (occurs_free e1) j (σ1' <{ xs1 ++ fvs ~> xs1 ++ ys' }>) rho1' rho3' *)
             rewrite extend_lst_app; [| reflexivity ].  
             eapply preord_env_P_inj_setlist_alt with (f := σ1 <{ fvs ~> ys' }>);
               [| eassumption | eassumption | eassumption | now eauto | | now eauto | now eauto ].
             + eapply preord_env_P_inj_resetlist; try eassumption.
-              * (* Disjoint M.elt (image σ1' (Setminus var (occurs_free e1) (FromList xs1)))
-                             (FromList ys') *)
-                eapply Disjoint_Included; [ | | now apply HDim ].
+              * eapply Disjoint_Included; [ | | now apply HDim ].
                 eapply Included_trans. eassumption. now eauto with Ensembles_DB.
                 apply image_monotonic. normalize_occurs_free.
                 apply Setminus_Included_Included_Union.
-                eapply Union_Included. eapply Included_trans. eassumption.
+                eapply Included_trans. eassumption.
                 now eauto 10 with Ensembles_DB.
-                now eauto with Ensembles_DB.
               * now eauto.
               * eapply preord_env_P_inj_antimon. eassumption.
                 normalize_occurs_free. apply Setminus_Included_Included_Union.
-                eapply Union_Included. eapply Included_trans. eassumption.
+                eapply Included_trans. eassumption.
                 now eauto 10 with Ensembles_DB.
-                now eauto with Ensembles_DB.
             + (* Disjoint var (image (σ1' <{ fvs ~> ys' }>)
                                        (Setminus var (occurs_free e1) (FromList xs1))) 
                             (FromList xs1) *)
@@ -1052,9 +1528,8 @@ Section Lambda_lifting_correct.
                 now eauto with Ensembles_DB.
                 apply image_monotonic. normalize_occurs_free.
                 do 2 apply Setminus_Included_Included_Union.
-                eapply Union_Included. eapply Included_trans. eassumption.
+                eapply Included_trans. eassumption.
                 now eauto 10 with Ensembles_DB.
-                now eauto with Ensembles_DB.
               * (* Disjoint var (FromList ys') (FromList xs1) *)
                 eapply Disjoint_Included_l; [ eassumption |].
                 eapply Disjoint_Included_l; [ eassumption |].
@@ -1063,12 +1538,10 @@ Section Lambda_lifting_correct.
           - rewrite extend_lst_app; [| reflexivity ].
             eapply Funs_inv_setlist; eauto.
             + eapply Funs_inv_setlist_getlist_r; eauto. 
-              * (* Disjoint var (LiftedFuns ζ1') (FromList ys') *)
-                now eauto with Ensembles_DB.
-              * eapply Disjoint_Included ; [ | | eapply HDim ].
-                eapply Included_trans. eapply Included_trans.
-                eassumption. eassumption. now eauto with Ensembles_DB.
-                apply image_monotonic...
+              eapply Disjoint_Included ; [ | | eapply HDim ].
+              eapply Included_trans. eassumption.
+              now eauto with Ensembles_DB.
+              apply image_monotonic...
             + (* Disjoint var (Funs ζ1') (FromList xs1) *)
               now eauto with Ensembles_DB.
             + (* Disjoint var (LiftedFuns ζ1') (FromList xs1) *)
@@ -1080,7 +1553,9 @@ Section Lambda_lifting_correct.
               * apply Union_Disjoint_l.
                 eapply Disjoint_Included; [ | | now apply HDim ].
                 now eauto with Ensembles_DB.
-                apply image_monotonic...
+                apply image_monotonic.
+                do 2 apply Setminus_Included_Included_Union.
+                now eauto 10 with Ensembles_DB.
                 eapply Disjoint_Included; [| | now apply Hf1 ].
                 eapply Included_Union_preserv_l. eassumption.
                 eapply Included_trans; eassumption.
@@ -1096,7 +1571,7 @@ Section Lambda_lifting_correct.
               eapply Fundefs_lambda_lift_name_in_fundefs in Hin'; [| eassumption ].
               inv Hin'. eapply Hf1. constructor.
               now eauto. left. now apply name_in_fundefs_bound_var_fundefs.
-              eapply Add_functions_LiftedFuns_Included in H; [| eassumption ].
+              eapply Add_functions_LiftedFuns_Included_r in H; [| eassumption ].
               inv H. eapply Hlf1. now constructor; eauto.
               now inv H0; eauto.
             + erewrite getlist_app. reflexivity.
@@ -1106,146 +1581,196 @@ Section Lambda_lifting_correct.
               rewrite FromList_map_image_FromList.
               eapply Disjoint_sym. eapply Disjoint_Included; [| | now apply HDim ].
               now eauto with Ensembles_DB.
-              apply image_monotonic.
-              eapply Included_trans. eassumption.
-              eapply Union_Included. normalize_occurs_free...
-              eapply Included_Union_preserv_l. eapply Included_Union_preserv_r.
-              eapply Included_trans; [| eapply Add_functions_FunsFVs_Included_l; eauto ].
-              reflexivity. eapply Disjoint_Included_r; [| eassumption ].
-              now apply name_in_fundefs_bound_var_fundefs. } }
+              apply image_monotonic. eapply Included_trans. eassumption.
+              apply Union_Included. normalize_occurs_free...
+              apply Union_Included. eapply Included_trans. 
+              eapply Add_functions_LiftedFuns_Included_l with (ζ' := ζ1); eauto.
+              eapply Disjoint_Included_r; [| eapply Hfun1 ].
+              eapply Included_Union_preserv_r.
+              now apply name_in_fundefs_bound_var_fundefs. now eauto with Ensembles_DB.
+              eapply Included_trans. eapply Add_functions_FunsFVs_Included_l.
+              now apply Hadd1. eassumption.
+              eapply Disjoint_Included_r; [| now apply Hfun1 ].
+              eapply Included_Union_preserv_r.
+              now apply name_in_fundefs_bound_var_fundefs.
+              now eauto with Ensembles_DB. } }
       split.
-      + eapply preord_env_P_inj_set_not_In_P_r; [ eapply preord_env_P_inj_set_alt |].
+      + assert (Heq : f' = f'0).
+         { rewrite Hfeq in H4. rewrite extend_gss in H4.
+           now inv H4. now left; eauto. } subst.
+        eapply preord_env_P_inj_set_extend_not_In_P_r;
+          [ eapply preord_env_P_inj_set_alt | | ].
         * eapply preord_env_P_inj_antimon. eassumption.
           now eauto 10 with Ensembles_DB.
         * eassumption.
         * intros Hc. eapply Add_functions_image_Included in Hc; [| eassumption ].
           inv Hc. eapply Him2. constructor; eauto. eapply image_monotonic; [| eassumption ].
           do 2 apply Setminus_Included_Included_Union.
-          apply Union_Included. now eauto 6 with Ensembles_DB.
-          eapply Included_trans. eapply Add_functions_FunsFVs_Included_r.
-          eassumption. apply Union_Included. now eauto with Ensembles_DB.
-          eapply Included_trans. eassumption. normalize_occurs_free...
-          normalize_bound_var...
-          eapply H9. now eapply name_in_fundefs_bound_var_fundefs.
+          apply Union_Included; now eauto 6 with Ensembles_DB.
+          inv H. eapply H9. now apply name_in_fundefs_bound_var_fundefs.
+          eapply Hf2. constructor; eauto. now eapply Setminus_Included; eauto.
+        * intros Hc. inv Hc. eapply Hf1. constructor; eauto.
+          now eapply Add_functions_free_set_Included; eauto.
+          eapply Hf2. constructor. now eapply Add_functions_free_set_Included; eauto.
+          left. rewrite bound_var_fundefs_Fcons. inv H; eauto.
+          do 3 right. now apply name_in_fundefs_bound_var_fundefs.
         * assert (Heqlf := lifted_name_eq _ _ _ _ _ H4).
           assert (Hinlf : In var (LiftedFuns ζ1) f'0) by (repeat eexists; eauto).
-          eapply Add_functions_LiftedFuns_Included in Hinlf; [| eassumption ]. 
-          intros Hc. eapply image_extend_Included' in Hc. inv Hc.
-          eapply Add_functions_image_Included in H; [| eassumption ].
-          inv H.
-          eapply Him2. constructor; eauto. eapply image_monotonic; [| eassumption ].
+          intros Hc. eapply image_extend_Included' in Hc. inv Hc. 
+          eapply Add_functions_image_Included in H; [| eassumption ]. inv H.
+          eapply Him2. constructor.
+          eapply image_monotonic; [| eassumption ].
           do 2 apply Setminus_Included_Included_Union.
-          apply Union_Included. now eauto 6 with Ensembles_DB.
-          eapply Included_trans. eapply Add_functions_FunsFVs_Included_r.
-          eassumption. apply Union_Included. now eauto with Ensembles_DB.
-          eapply Included_trans. eassumption. normalize_occurs_free...
-          inv Hinlf. now eauto. left. eapply Setminus_Included. eassumption.
-          inv Hinlf. eapply Hlf2. constructor; eauto.
-          right. normalize_bound_var. do 3 right. now apply name_in_fundefs_bound_var_fundefs.
-          eapply Hf2 with (x := f'0). constructor; eauto.
-          eapply Setminus_Included. eassumption.
-          left. normalize_bound_var. do 3 right. now apply name_in_fundefs_bound_var_fundefs.
-          inv H. inv Hinlf.
-          eapply Hlf2. now constructor; eauto.
-          eapply Hf2. constructor; eauto. eapply Setminus_Included. eassumption.
+          now eauto 10 with Ensembles_DB.
+          left. eapply Add_functions_free_set_Included; eassumption.
+          inv H0. eapply Hf2. constructor.
+          eapply Add_functions_free_set_Included; eassumption.
+          left. normalize_bound_var. do 3 right.
+          now apply name_in_fundefs_bound_var_fundefs. now inv H; eauto.
+          inv H; subst. eapply Hf2.
+          constructor; eauto. eapply Add_functions_free_set_Included; eassumption.
       + edestruct name_in_fundefs_find_def_is_Some as [ft1 [xs1 [e1 Hdef]]].
         apply Hinc. now left.
         edestruct Fundefs_lambda_lift_find_def with (B1 := B1)
           as (xs2 & ys' & e2 & S3 & S2 & Hfind1 & Hfind2 & Hnd1
                   & Hnd2 & Hlen1 & Hlen2 & Hinc1' & Hinc2' & Hinc3' & HD1' & HD2' & HD3' & Hll);
         try eassumption.
-        eapply Disjoint_Included_r_sym. eapply Add_functions_LiftedFuns_Included. eassumption.
+        eapply Disjoint_Included_r_sym. eapply Add_functions_LiftedFuns_Included_r. eassumption.
         eapply Union_Disjoint_l. eapply Disjoint_Included_r; [| now apply Hlf1 ]...
         eapply Disjoint_Included; [| | now apply Hf1]...
         eapply Add_functions_injective_subdomain_LiftedFuns. eassumption.
         assert (Hinc' : Included M.elt (FromList fvs0)
-                                (Union var (occurs_free (Efun B1 e)) (FunsFVs ζ))).
+                                (Union var (occurs_free (Efun B1 e)) (Union _ (LiftedFuns ζ) (FunsFVs ζ)))).
         { eapply Included_trans with (s2 := FunsFVs ζ1).
           intros x Hx. now repeat eexists; eauto. 
           eapply Included_trans. eapply Add_functions_FunsFVs_Included_r. eassumption.
           eapply Included_trans. apply Included_Union_compat. reflexivity. eassumption.
-          normalize_occurs_free... }
-        assert (HDfvs :  Disjoint var (FromList fvs0) (name_in_fundefs B1)).
-        { eapply Disjoint_Included_l with (s3 := (FunsFVs ζ1)).
+          normalize_occurs_free. now eauto 10 with Ensembles_DB. }
+        assert (HDfvs :  Disjoint var (FromList fvs0)
+                                  (Union _  (name_in_fundefs B1) (Setminus var S S1'))).
+        { clear Hlf2 Hfvs2.
+          eapply Disjoint_Included_l with (s3 := (FunsFVs ζ1)).
           eexists; eauto.
           eapply Disjoint_Included_l. eapply Add_functions_FunsFVs_Included_r.
           eassumption.
-          eapply Disjoint_Included_r. now apply name_in_fundefs_bound_var_fundefs.
-          now eauto with Ensembles_DB. }
-        assert (HDfvs' :  Disjoint var (FromList fvs0) (name_in_fundefs B2)).
-        { eapply Disjoint_Included_l with (s3 := (FunsFVs ζ1)).
-          eexists; eauto.
-          eapply Disjoint_Included_l. eapply Add_functions_FunsFVs_Included_r.
-          eassumption.
-          eapply Disjoint_Included_r. now apply name_in_fundefs_bound_var_fundefs.
-          rewrite !bound_var_fundefs_Fcons in Hfvs2, HD2.
+          eapply Disjoint_Included_r.
+          eapply Included_Union_compat. now apply name_in_fundefs_bound_var_fundefs.
+          now apply Setminus_Included.
+          apply Union_Disjoint_l. now eauto with Ensembles_DB.
+          eapply Disjoint_Included_l. eassumption. eapply Union_Disjoint_l.
+          eapply Disjoint_sym. eapply Union_Disjoint_l. eassumption.
+          eapply Disjoint_Included; [| | eapply Hf1 ]. normalize_occurs_free...
+          reflexivity.
           eapply Union_Disjoint_l; now eauto with Ensembles_DB. }
+        assert (HDfvs' :  Disjoint var (FromList fvs0)
+                                   (Union _  (name_in_fundefs B2) (Setminus var S S'))).
+        { eapply Disjoint_Included_l with (s3 := (FunsFVs ζ1)).
+          eexists; eauto.
+          eapply Disjoint_Included_l. eapply Add_functions_FunsFVs_Included_r.
+          eassumption. eapply Union_Disjoint_l.
+          eapply Disjoint_Included_r; [| eassumption ].
+          eapply Included_trans. apply Included_Union_compat. now apply name_in_fundefs_bound_var_fundefs.
+          now apply Setminus_Included. normalize_bound_var...
+          eapply Disjoint_Included_r; [| eassumption ].
+          eapply Included_trans. apply Included_Union_compat. now apply name_in_fundefs_bound_var_fundefs.
+          now apply Setminus_Included. normalize_bound_var... }
         assert (Ha1 : @map var var  σ1 fvs0 = map σ fvs0).
         { symmetry. eapply Add_functions_map_eq; eassumption. }
         assert (Ha2 : @map var var σ' fvs0 = map σ fvs0).
         { symmetry. eapply Add_functions_map_eq; eassumption. }
-        edestruct (@binding_in_map_getlist val) with (xs := fvs0) as [vs Hget]; eauto.
-        edestruct preord_env_P_inj_getlist_l as [vs2' [Hgetfvs' Hprefvs]]. now apply Henv.
-        eassumption. eassumption.
+        edestruct (@binding_in_map_getlist val) with (xs := (map σ1 fvs0)) as [vs Hget]; eauto.
+        rewrite Ha1. rewrite FromList_map_image_FromList. eapply image_monotonic.
+        eapply Included_trans. eassumption. now eauto with Ensembles_DB.
         rewrite Hfeq in H4. rewrite extend_gss in H4. inv H4.
         rewrite Ha1, <- Ha2 in Hfind1. 
         eapply Funs_inv_set_lifted; (try now apply H4); eauto.
-        * rewrite Ha2. 
-          rewrite getlist_def_funs_Disjoint. eassumption.
+        * rewrite (Add_functions_Fundefs_lambda_lift_name_in_fundefs B1 B1')...
+        * rewrite Ha2.
+          rewrite getlist_def_funs_Disjoint. rewrite <- Ha1. eassumption.
+          simpl in Hfeq. rewrite Union_commut in Hfeq.
+          apply f_eq_subdomain_extend_not_In_S_r' in Hfeq.
+          rewrite (Add_functions_Fundefs_lambda_lift_name_in_fundefs B2 B'); [| now eauto | | | ]; eauto.
           rewrite FromList_map_image_FromList.
           eapply Disjoint_Included; [| | now apply Him2 ].
-          eapply Included_trans.
-          eapply Fundefs_lambda_lift_name_in_fundefs. eassumption.
-          eapply Included_trans. apply Included_Union_compat.
-          apply name_in_fundefs_bound_var_fundefs.
-          eapply Add_functions_LiftedFuns_Included. eassumption.
-          normalize_bound_var; now eauto 9 with Ensembles_DB.
-          apply image_monotonic. eassumption.
+          eapply Included_trans. rewrite Union_commut.
+          eapply Included_Union_compat. reflexivity.
+          now apply name_in_fundefs_bound_var_fundefs.
+          normalize_bound_var...
+          apply image_monotonic. eapply Included_trans. eassumption.
+          normalize_occurs_free... symmetry; eassumption.
+          intros Hc. eapply H9. now apply name_in_fundefs_bound_var_fundefs.
         * congruence.
-        * eapply Union_Disjoint_l; [| eassumption ].
+        * eapply Union_Disjoint_l.
           eapply Disjoint_Included_l.
           eapply Add_functions_FunsFVs_Included_r. eassumption.
-          apply Union_Disjoint_l. now eauto with Ensembles_DB.
-          eassumption.
+          apply Union_Disjoint_l. clear Hfvs2. now eauto with Ensembles_DB.
+          eapply Disjoint_Included_l. eassumption.
+          eapply Union_Disjoint_l. eapply Disjoint_sym. eassumption.
+          clear Hlf2 Hfvs2. now eauto with Ensembles_DB.
+          clear HD2. now eauto with Ensembles_DB.
         * clear Hlf2 Hf2. 
           eapply Disjoint_Included_l.
-          eapply Add_functions_LiftedFuns_Included. eassumption.
+          eapply Add_functions_LiftedFuns_Included_r. eassumption.
           apply Union_Disjoint_l. now eauto with Ensembles_DB.
           eapply Disjoint_Included_l. now apply Setminus_Included.
           now eauto with Ensembles_DB.
-        * eapply Disjoint_Included_l with (s3 := image σ (Union var (FromList fvs0) (FunsFVs ζ'))).
-          rewrite <- image_f_eq_subdomain. reflexivity.
-          eapply f_eq_subdomain_antimon; [| eapply Add_functions_σ_eq; eauto ].
-          eapply Included_trans.
+        * unfold LiftedFuns. 
+          rewrite Add_functions_Funs_Same_set; eauto.
+          rewrite image'_Union, Add_functions_name_in_fundefs; eauto.
+          rewrite Add_functions_lifted_name_Disjoint_Same_set; eauto.
+          rewrite image_Union.
+          rewrite Add_functions_image_Disjoint_Same_set, Add_functions_image_LiftedFuns_Same_set; eauto.
+          eapply Union_Disjoint_l.
+          eapply Disjoint_Included; [| | now apply Him1 ]. 
+          eapply Included_Union_preserv_r. now apply name_in_fundefs_bound_var_fundefs.
+          eapply image_monotonic...
+          eapply Disjoint_Included; [| | now apply Hf1 ].
+          eapply Included_Union_preserv_l. now apply name_in_fundefs_bound_var_fundefs.
+          now eauto with Ensembles_DB.
+          eapply Disjoint_Included_r; [| now apply Hf2 ].
+          eapply Included_trans; [now apply name_in_fundefs_bound_var_fundefs | ].
+          normalize_bound_var...
+          eapply Disjoint_Included_r; [| now apply Hlf2 ].
           eapply Included_Union_compat. reflexivity.
-          eapply Add_functions_FunsFVs_Included_r. eassumption.
-          intros x Hx Hc. apply name_in_fundefs_bound_var_fundefs in Hc. inv Hx.
-          eapply HD2. now constructor; eauto.
-          inv H. eapply Hfvs2. now constructor; eauto.
-          eapply HD2. now constructor; eauto.
-          eapply Disjoint_Included_l. 
-          apply image_monotonic. eapply Included_Union_compat. reflexivity.
-          eapply Add_functions_FunsFVs_Included_r. eassumption.
-          eapply Disjoint_Included_r. apply Included_Union_compat.
-          eapply Included_trans. eapply Fundefs_lambda_lift_name_in_fundefs.
-          eassumption. apply Included_Union_compat. now apply name_in_fundefs_bound_var_fundefs.
-          eapply Add_functions_LiftedFuns_Included. eassumption.
-          eapply Included_trans. eapply Included_trans; eassumption.
-          eapply Add_functions_free_set_Included. eassumption.
-          rewrite image_Union. 
-          apply Union_Disjoint_l.
-          eapply Disjoint_Included; [| | now apply Him1 ].
-          now eauto 7 with Ensembles_DB. apply image_monotonic...
-          eapply Disjoint_Included; [| | now apply Him1 ].
-          now eauto 7 with Ensembles_DB.
-          apply image_monotonic. eapply Included_trans.
-          eapply Included_Union_compat. reflexivity. eassumption.
-          normalize_occurs_free...        
+          eapply Included_trans; [now apply name_in_fundefs_bound_var_fundefs | ].
+          normalize_bound_var...
+          eapply Disjoint_Included_r; [| now apply Hfun2 ].
+          eapply Included_Union_compat. reflexivity.
+          normalize_bound_var. do 3 eapply Included_Union_preserv_r.
+          now apply name_in_fundefs_bound_var_fundefs.
+        * rewrite image_Union.
+          rewrite <- FromList_map_image_FromList, Ha2, FromList_map_image_FromList.
+          rewrite (Add_functions_Fundefs_lambda_lift_name_in_fundefs B1 B1'); [ | now eauto | | | ]; eauto; try reflexivity.
+          rewrite Add_functions_image_Disjoint_Same_set with (σ' := σ'); eauto.
+          eapply Disjoint_Included_r with (s2 := Union var S (name_in_fundefs B1)).
+          eapply Union_Included; [ eapply Union_Included |]; eauto with Ensembles_DB.
+          eapply Included_trans. eassumption.
+          eapply Included_trans. eassumption.
+          eapply Included_trans. now eapply Add_functions_free_set_Included; eauto.
+          now eauto with Ensembles_DB.
+          rewrite <- image_Union. eapply Disjoint_Included; [| |  now apply Him1].
+          eapply Included_Union_compat. reflexivity.
+          now apply name_in_fundefs_bound_var_fundefs.
+          eapply image_monotonic. eapply Union_Included.
+          eapply Included_trans. eassumption. normalize_occurs_free...
+          eapply Included_trans. eapply Add_functions_FunsFVs_Included_r.
+          eassumption. eapply Union_Included. now eauto with Ensembles_DB.
+          eapply Included_trans. eassumption. normalize_occurs_free...
+          eapply Disjoint_Included_l. eapply Add_functions_FunsFVs_Included_r.
+          eassumption. eapply Union_Disjoint_l.
+          eapply Disjoint_Included_r; [| eassumption ].
+          eapply Included_Union_compat. reflexivity.
+          eapply Included_trans. now apply name_in_fundefs_bound_var_fundefs.
+          normalize_bound_var...
+          eapply Disjoint_Included_r; [| eassumption ].
+          eapply Included_Union_compat. reflexivity.
+          eapply Included_trans. now apply name_in_fundefs_bound_var_fundefs.
+          normalize_bound_var...
         * eapply Disjoint_Included_r.
           eapply Included_trans.
           eapply Fundefs_lambda_lift_name_in_fundefs. eassumption.
           apply Included_Union_compat. now apply name_in_fundefs_bound_var_fundefs.
-          eapply Add_functions_LiftedFuns_Included. eassumption.
+          eapply Add_functions_LiftedFuns_Included_r. eassumption.
           eapply Disjoint_Included_l.
           eapply Included_trans; eassumption.
           rewrite Union_assoc. apply Union_Disjoint_r.
@@ -1253,34 +1778,46 @@ Section Lambda_lifting_correct.
           eapply Add_functions_free_set_Included. eassumption.
           clear Hf2...
           now eauto with Ensembles_DB.
-        * intros Hc.
-          eapply Add_functions_LiftedFuns_Included in Hc; [| eassumption ].
-          inv Hc. eapply Hlf1. constructor; eauto.
-          left. eapply Add_functions_free_set_Included; eassumption.
-          inv H; eauto.
-        * eapply preord_env_P_inj_antimon. eassumption.
-          eapply Included_trans. eassumption.
-          eapply Union_Included. normalize_occurs_free...
-          eapply Included_trans.
-          eapply Add_functions_FunsFVs_Included_l with (ζ' := ζ1); eauto.
-          eapply Disjoint_Included_r; [| eassumption ].
+        * eapply Disjoint_Included_l.
+          now eapply Add_functions_FunsFVs_Included_r; eauto.
+          rewrite Add_functions_Fundefs_lambda_lift_name_in_fundefs; [| | now eauto | | ]; eauto.
+          eapply Union_Disjoint_l.
+          eapply Disjoint_Included_r; [| now apply Hfvs1 ]. rewrite Union_commut.
+          apply Included_Union_compat. now eauto with Ensembles_DB.
           now apply name_in_fundefs_bound_var_fundefs.
-          now eauto with Ensembles_DB.
+          eapply Disjoint_Included_r; [| now apply HD1 ]. rewrite Union_commut.
+          apply Included_Union_compat. now eauto with Ensembles_DB.
+          now apply name_in_fundefs_bound_var_fundefs.
+          reflexivity.
+        * intros Hc. eapply Add_functions_LiftedFuns_Included_r in Hc; [| eassumption ].
+          inv Hc. eapply Hlf1. constructor; eauto. left.
+          now eapply Add_functions_free_set_Included; eauto.
+          now inv H; eauto.
+        * intros Hc. eapply HD1. constructor; eauto. left.
+          now eapply Add_functions_free_set_Included; eauto.
+        * intros Hc.
+          eapply image_monotonic in Hc;
+            [| eapply Add_functions_LiftedFuns_Included_r ; now eauto ].
+          eapply Add_functions_image_Included in Hc; eauto. inv Hc.
+          rewrite Setminus_Union_distr in H.
+          rewrite (Setminus_Included_Empty_set (Setminus var S S')) in H;
+            try eauto with Ensembles_DB.
+          rewrite Union_Empty_set_neut_r in H. eapply Him2.
+          constructor. eapply image_monotonic; [| eassumption ]...
+          left. now eapply Add_functions_free_set_Included; eauto.
+          inv H. eapply Hf2. constructor.
+          now eapply Add_functions_free_set_Included; eauto.
+          left. rewrite bound_var_fundefs_Fcons. do 3 right.
+          now apply name_in_fundefs_bound_var_fundefs.
+          now inv H0; eauto.
         * left; eauto.
     - inv Hll2. inv Hadd2. simpl. rewrite Union_Empty_set_neut_r.
-      split; eauto.
-      eapply preord_env_P_inj_antimon. eassumption.
-      eapply Included_trans.
-      eapply Included_Union_compat. reflexivity.
-      eapply Included_trans. eapply Add_functions_FunsFVs_Included_r.
-      eassumption.
-      eapply Included_Union_compat. reflexivity. eassumption.
-      intros x Hin'. inv Hin'; eauto. inv H; eauto. inv H0; eauto.
+      split; eauto. 
   Qed.
 
   Corollary Fundefs_lambda_lift_correct_cor k rho rho' B1 B1' σ ζ σ1 ζ1 S
-        S1' S1'' S1''' fvs e:
-    (* The IH for expressions *)
+            S1' S1'' S1''' fvs e:
+        (* The IH for expressions *)
      (forall m : nat,
         m < k ->
         forall (e : exp) (rho rho' : env)
@@ -1288,15 +1825,15 @@ Section Lambda_lifting_correct.
           (σ : var -> var) (S : Ensemble var) (e' : exp) 
           (S' : Ensemble var),
         unique_bindings e ->
-        Disjoint var (image σ (Union _ (occurs_free e) (FunsFVs ζ)))
-                 (Union var S (Union _ (bound_var e) (LiftedFuns ζ))) ->
+        Disjoint var (image σ (Union _ (Union _ (occurs_free e) (FunsFVs ζ)) (LiftedFuns ζ)))
+                 (Union var S (bound_var e)) ->
         Disjoint var S (Union var (bound_var e) (occurs_free e)) ->
         Disjoint var (LiftedFuns ζ) (Union _ S (bound_var e)) ->
-        Disjoint var (Funs ζ) (bound_var e) ->
-        Disjoint var (FunsFVs ζ) (bound_var e) ->
+        Disjoint var (Funs ζ) (Union _ S (bound_var e)) ->
+        Disjoint var (FunsFVs ζ) (Union _ S (bound_var e)) ->
         Disjoint _ (bound_var e) (occurs_free e) ->
-        binding_in_map (Union _ (occurs_free e) (FunsFVs ζ)) rho ->
-        preord_env_P_inj pr cenv (Union _ (occurs_free e) (FunsFVs ζ)) m σ rho rho' ->
+        binding_in_map (image σ (Union _ (Union _ (occurs_free e) (FunsFVs ζ)) (LiftedFuns ζ))) rho' ->
+        preord_env_P_inj pr cenv (occurs_free e) m σ rho rho' ->
         Funs_inv m rho rho' σ ζ ->
         Exp_lambda_lift ζ σ e S e' S' ->
         preord_exp pr cenv m (e, rho) (e', rho')) ->
@@ -1305,45 +1842,47 @@ Section Lambda_lifting_correct.
      unique_bindings_fundefs B1 ->
 
      (* The image of σ is neither in the free set nor in the set of bound variables *)
-     Disjoint var (image σ (Union _ (occurs_free (Efun B1 e)) (FunsFVs ζ)))
-              (Union var S (Union _ (bound_var_fundefs B1) (LiftedFuns ζ))) ->
+     Disjoint var (image σ (Union _ (occurs_free (Efun B1 e)) (Union _ (FunsFVs ζ) (LiftedFuns ζ))))
+              (Union var S (bound_var_fundefs B1)) ->
 
      (* The free set is disjoint from the set of bound and free variables *)
-     Disjoint var S (Union var (bound_var_fundefs B1) (occurs_free_fundefs B1)) ->
+     Disjoint var S (Union var (bound_var_fundefs B1) (occurs_free (Efun B1 e))) ->
 
      (* The names of lifted functions is neither in the free set nor in the set of bound variables*) 
      Disjoint var (LiftedFuns ζ) (Union _ S (bound_var_fundefs B1)) ->
 
      (* The domain of ζ is disjoint with the bound variables *)
-     Disjoint var (Funs ζ) (bound_var_fundefs B1) ->
+     Disjoint var (Funs ζ) (Union _ S (bound_var_fundefs B1)) ->
 
      (* The free variables of the funs in ζ are disjoint from the bound variables *) 
-     Disjoint var (FunsFVs ζ) (bound_var_fundefs B1) ->
+     Disjoint var (FunsFVs ζ) (Union _ S (bound_var_fundefs B1)) ->
 
-     (* The free and bound variables are disjoint *)
+     (* The bound variables and the free variables are disjoint *)
      Disjoint _ (bound_var_fundefs B1) (occurs_free_fundefs B1) ->
 
-     (* All the free variables are in the map *)
-     binding_in_map (Union _ (occurs_free (Efun B1 e)) (FunsFVs ζ)) rho ->
+     (* The free variables are in the environment *)
+     binding_in_map (image σ (Union _ (occurs_free (Efun B1 e)) (Union _ (FunsFVs ζ) (LiftedFuns ζ))))
+                    rho' ->
 
-     (* The invariants hold in the initial environment *)
-     preord_env_P_inj pr cenv (Union _ (occurs_free (Efun B1 e)) (FunsFVs ζ)) k σ rho rho' ->
+     (** The invariants hold for the initial environments **)
+     preord_env_P_inj pr cenv (occurs_free (Efun B1 e)) k σ rho rho' ->
      Funs_inv k rho rho' σ ζ ->
      
      NoDup fvs ->
-     Included _ (FromList fvs) (Union _ (occurs_free_fundefs B1) (FunsFVs ζ)) ->
-     Disjoint var (FromList fvs) (bound_var_fundefs B1) ->
+     Included _ (FromList fvs) (Union _ (occurs_free_fundefs B1) (Union _ (LiftedFuns ζ) (FunsFVs ζ))) ->
+     Disjoint var (FromList fvs) (Union _ S (bound_var_fundefs B1)) ->
      
      Add_functions B1 fvs σ ζ S σ1 ζ1 S1' ->
      Included _ S1'' S1' ->
      Fundefs_lambda_lift ζ1 σ1 B1 S1'' B1' S1''' ->
-     
-     (* The invariants hold in the final environment *)
-     preord_env_P_inj pr cenv (Union _ (Union _ (occurs_free (Efun B1 e)) (name_in_fundefs B1)) (FunsFVs ζ1))
+
+     (** The invariants hold for the final environments **)
+     preord_env_P_inj pr cenv (Union _ (occurs_free (Efun B1 e)) (name_in_fundefs B1))
                       k σ1 (def_funs B1 B1 rho rho) (def_funs B1' B1' rho' rho') /\
      Funs_inv k (def_funs B1 B1 rho rho) (def_funs B1' B1' rho' rho') σ1 ζ1.
-  Proof.
+  Proof with now eauto with Ensembles_DB.
     intros. eapply Fundefs_lambda_lift_correct; eauto.
+    eapply Disjoint_Included_r; [| eassumption ]. normalize_occurs_free...
     reflexivity. reflexivity.
   Qed.
 
@@ -1362,22 +1901,22 @@ Section Lambda_lifting_correct.
     (* The expression has unique bindings *)
     unique_bindings e ->
     (* The new free variable names are fresh *)
-    Disjoint _ (image σ (Union _ (occurs_free e) (FunsFVs ζ)))
-             (Union _ S (Union _ (bound_var e) (LiftedFuns ζ))) ->
+    Disjoint var (image σ (Union _ (Union _ (occurs_free e) (FunsFVs ζ)) (LiftedFuns ζ)))
+             (Union var S (bound_var e)) ->
     (* The fresh set is fresh *)
     Disjoint _ S (Union _ (bound_var e) (occurs_free e)) ->
     (* The new function names for lifted functions are fresh *)
     Disjoint _ (LiftedFuns ζ) (Union _ S (bound_var e)) ->
     (* The names of the (already defined) functions are disjoint from the bound variables of the expression *)
-    Disjoint _ (Funs ζ) (bound_var e) ->
+    Disjoint var (Funs ζ) (Union _ S (bound_var e)) ->
     (* The free variables of a function are disjoint from the bound variables of the expression *)
-    Disjoint _ (FunsFVs ζ) (bound_var e) ->
+    Disjoint var (FunsFVs ζ) (Union _ S (bound_var e)) ->    
     (* The bound variables of the expression are disjoint from the free variables *)
     Disjoint _ (bound_var e) (occurs_free e) ->
     (* All the free variables are in the environment *)
-    binding_in_map (Union _ (occurs_free e) (FunsFVs ζ)) rho ->
+    binding_in_map (image σ (Union _ (Union _ (occurs_free e) (FunsFVs ζ)) (LiftedFuns ζ))) rho' ->
     (* The environments are related *)
-    preord_env_P_inj pr cenv (Union _ (occurs_free e) (FunsFVs ζ)) k σ rho rho' ->
+    preord_env_P_inj pr cenv (occurs_free e) k σ rho rho' ->
     (* The invariant about lifted functions hold*)
     Funs_inv k rho rho' σ ζ ->
     (* e' is the translation of e*)
@@ -1398,11 +1937,11 @@ Section Lambda_lifting_correct.
           rewrite occurs_free_Econstr in Him.
           eapply Disjoint_Included; [ | | now apply Him ].
           normalize_bound_var...
-          apply image_monotonic. rewrite Setminus_Union_distr...
+          apply image_monotonic.
+          rewrite !Setminus_Union_distr...
           eapply Union_Disjoint_r.
           eapply Disjoint_Included_l_sym; [| eassumption ]...
-          eapply Disjoint_Singleton_l. intros Hc. inv Hc. now eauto.
-          eapply Hlf. now constructor; eauto.
+          eapply Disjoint_Singleton_l. intros Hc. now eauto.
         * eapply Disjoint_Included_r; [| eassumption ].
           now apply bound_var_occurs_free_Econstr_Included.
         * repeat normalize_bound_var_in_ctx...
@@ -1413,20 +1952,18 @@ Section Lambda_lifting_correct.
           eapply Disjoint_Included_l ; [| now apply HD].
           normalize_bound_var... now apply Disjoint_Singleton_r.
         * eapply binding_in_map_antimon; [| eapply binding_in_map_set; eassumption ]. 
-          apply Union_Included; [| now eauto with Ensembles_DB ].
-          rewrite Union_commut, Union_assoc.
-          apply Included_Union_preserv_l.
-          normalize_occurs_free. rewrite Union_assoc.
-          rewrite Union_Setminus_Included;
-            now eauto with Ensembles_DB typeclass_instances.
+          eapply Included_trans. eapply image_extend_Included'.
+          eapply Included_Union_compat; [| reflexivity ].
+          eapply image_monotonic. rewrite !Setminus_Union_distr.
+          normalize_occurs_free...
         * eapply preord_env_P_inj_set_alt.
           eapply preord_env_P_inj_antimon. eassumption.
-          rewrite Setminus_Union_distr; normalize_occurs_free...
+          normalize_occurs_free...
           rewrite preord_val_eq. constructor. reflexivity.
           now apply Forall2_Forall2_asym_included.
           intros Hc. eapply Him. constructor; eauto.
           eapply image_monotonic; [| eassumption ].
-          rewrite Setminus_Union_distr; normalize_occurs_free...
+          normalize_occurs_free...
         * eapply Funs_inv_set.
           intros Hc. eapply Hfun. now constructor; eauto.
           intros Hc. eapply Hlf. now constructor; eauto.
@@ -1437,7 +1974,6 @@ Section Lambda_lifting_correct.
     - eapply preord_exp_case_nil_compat.
     - inv Hun. edestruct Exp_lambda_lift_Ecase as [P'' [Heq Hall]]; eauto. inv Heq.
       eapply preord_exp_case_cons_compat; eauto.
-      + eapply Henv. left; eauto.
       + eapply IHe; eauto.
         * eapply Disjoint_Included; [| | now apply Him ].
           normalize_bound_var...
@@ -1477,18 +2013,17 @@ Section Lambda_lifting_correct.
         * eapply preord_env_P_inj_antimon. eassumption.
           normalize_occurs_free...
     - inv Hun. eapply preord_exp_proj_compat.
-      + eapply Henv. left. normalize_occurs_free...
+      + eapply Henv. eauto.
       + intros vs1 vs2 Hall. eapply IHe; [ eassumption | | | | | | | | | | eassumption ].
         * eapply Disjoint_Included_l. now eapply image_extend_Included'.
           eapply Union_Disjoint_l.
           rewrite occurs_free_Eproj in Him.
           eapply Disjoint_Included; [ | | now apply Him ].
           normalize_bound_var...
-          apply image_monotonic. rewrite Setminus_Union_distr...
+          apply image_monotonic. rewrite !Setminus_Union_distr...
           eapply Union_Disjoint_r.
           eapply Disjoint_Included_l_sym; [| eassumption ]...
-          eapply Disjoint_Singleton_l. intros Hc. inv Hc. now eauto.
-          eapply Hlf. now constructor; eauto.
+          now eapply Disjoint_Singleton_l.
         * eapply Disjoint_Included_r; [| eassumption ].
           now apply bound_var_occurs_free_Eproj_Included.
         * repeat normalize_bound_var_in_ctx...
@@ -1498,20 +2033,17 @@ Section Lambda_lifting_correct.
           eapply Union_Disjoint_r.
           eapply Disjoint_Included_l ; [| now apply HD].
           normalize_bound_var... now apply Disjoint_Singleton_r.
-        * eapply binding_in_map_antimon; [| eapply binding_in_map_set; eassumption ]. 
-          apply Union_Included; [| now eauto with Ensembles_DB ].
-          rewrite Union_commut, Union_assoc.
-          apply Included_Union_preserv_l.
-          normalize_occurs_free. rewrite Union_assoc.
-          rewrite Union_Setminus_Included;
-            now eauto with Ensembles_DB typeclass_instances.
+        * eapply binding_in_map_antimon; [| eapply binding_in_map_set; eassumption ].
+          eapply Included_trans. eapply image_extend_Included'.
+          eapply Included_Union_compat; [| reflexivity ].
+          eapply image_monotonic. rewrite !Setminus_Union_distr.
+          normalize_occurs_free...
         * eapply preord_env_P_inj_set_alt.
           eapply preord_env_P_inj_antimon. eassumption.
-          rewrite Setminus_Union_distr; normalize_occurs_free...
-          eassumption.
+          normalize_occurs_free... eassumption.
           intros Hc. eapply Him. constructor; eauto.
           eapply image_monotonic; [| eassumption ].
-          rewrite Setminus_Union_distr; normalize_occurs_free...
+          normalize_occurs_free...
         * eapply Funs_inv_set.
           intros Hc. eapply Hfun. now constructor; eauto.
           intros Hc. eapply Hlf. now constructor; eauto.
@@ -1526,44 +2058,61 @@ Section Lambda_lifting_correct.
       inv Hun. eapply preord_exp_fun_compat.
       repeat normalize_bound_var_in_ctx.
       edestruct Fundefs_lambda_lift_correct_cor; eauto; eauto with Ensembles_DB.
-      + eapply Disjoint_Included_r; [| now apply Hf ].
-        rewrite <- bound_var_Efun.
-        now apply bound_var_occurs_free_fundefs_Efun_Included.
+      + eapply Disjoint_Included; [ | | now apply Him ].
+        now eauto with Ensembles_DB.
+        rewrite Union_assoc...
       + eapply Disjoint_Included; [| | now apply HD].
         normalize_occurs_free... now eauto with Ensembles_DB.
+      + eapply binding_in_map_antimon ; [| eassumption ].
+        rewrite Union_assoc...
+      + eapply Included_trans; [ eassumption |]...
       + eapply Disjoint_Included_l. eassumption. eapply Union_Disjoint_l.
-        apply Disjoint_sym. eapply Disjoint_Included; [| | now apply HD ].
+        eapply Union_Disjoint_r.
+        rewrite occurs_free_Efun in Hf...
+        eapply Disjoint_sym. eapply Disjoint_Included; [| | now apply HD ].
         normalize_occurs_free... now eauto with Ensembles_DB.
+        eapply Union_Disjoint_l.
+        eapply Disjoint_Included_r; [| eassumption ]...
         eapply Disjoint_Included_r; [| eassumption ]...
       + eapply IHe; eauto.
-        * eapply Disjoint_Included_r.
-          apply Included_Union_compat. eassumption.
+        * eapply Disjoint_Included_l. 
+          eapply image_monotonic. eapply Included_Union_compat.
           eapply Included_Union_compat. reflexivity.
-          eapply Add_functions_LiftedFuns_Included. eassumption.
-          eapply Disjoint_Included_l. 
-          eapply Add_functions_image_Included. eassumption.
-          apply Union_Disjoint_l.
-          eapply Disjoint_Included; [| | now apply Him ].
-          now eauto 10 with Ensembles_DB.
-          apply image_monotonic. rewrite Setminus_Union_distr.
-          eapply Union_Included. normalize_occurs_free...
-          apply Setminus_Included_Included_Union. normalize_occurs_free.
-          eapply Included_trans. eapply Add_functions_FunsFVs_Included_r.
+          eapply Add_functions_FunsFVs_Included_r. eassumption.
+          eapply Add_functions_LiftedFuns_Included_r. eassumption.
+          eapply Disjoint_Included_l. eapply Add_functions_image_Included.
           eassumption.
-          eapply Union_Included. now eauto with Ensembles_DB.
-          eapply Included_trans; [ eassumption |]...
-          eapply Disjoint_Included_l. now apply name_in_fundefs_bound_var_fundefs. 
-          apply Union_Disjoint_r. now eauto with Ensembles_DB.
-          apply Union_Disjoint_r. now eauto with Ensembles_DB.
-          apply Union_Disjoint_r. now eauto with Ensembles_DB.
-          eapply Disjoint_Included_r. now apply Setminus_Included.
+          apply Union_Disjoint_l.
+          eapply Disjoint_Included_r. eapply Included_Union_compat.
+          eassumption. reflexivity.
+          eapply Disjoint_Included; [| | now apply Him ].
           now eauto with Ensembles_DB.
+          apply image_monotonic. rewrite !Setminus_Union_distr.
+          rewrite (Setminus_Included_Empty_set (Setminus var S S'0)), Union_Empty_set_neut_r.
+          eapply Union_Included. eapply Union_Included. 
+          rewrite <- Setminus_Union. normalize_occurs_free...
+          eapply Union_Included. now eauto with Ensembles_DB.
+          eapply Included_trans. eapply Included_Setminus_compat.
+          eassumption. reflexivity. rewrite !Setminus_Union_distr.
+          eapply Union_Included. 
+          rewrite <- Setminus_Union. normalize_occurs_free...
+          now eauto with Ensembles_DB. now eauto with Ensembles_DB.
+          now eauto with Ensembles_DB.
+          eapply Union_Disjoint_l.
+          eapply Disjoint_Included_l. now apply name_in_fundefs_bound_var_fundefs.                     
+          apply Union_Disjoint_r.
+          eapply Disjoint_sym. eapply Disjoint_Included; [| | now apply Hf ].
+          now eauto with Ensembles_DB. eassumption.
+          now eapply Disjoint_sym.
+          apply Union_Disjoint_r. eapply Disjoint_Setminus_l.
+          eapply Fundefs_Lambda_lift_free_set_Included. eassumption.
+          eapply Disjoint_Included; [| | now apply Hf ]...
         * eapply Disjoint_Included; [| | now apply Hf ].
           rewrite <- bound_var_Efun.
           now apply bound_var_occurs_free_Efun_Included.
           eassumption.
         * eapply Disjoint_Included_l.
-          eapply Add_functions_LiftedFuns_Included. eassumption.
+          eapply Add_functions_LiftedFuns_Included_r. eassumption.
           apply Union_Disjoint_l. now eauto with Ensembles_DB.
           apply Union_Disjoint_r.
           eapply Disjoint_Included_r. eapply Fundefs_Lambda_lift_free_set_Included.
@@ -1572,16 +2121,22 @@ Section Lambda_lifting_correct.
         * eapply Disjoint_Included_l.
           eapply Add_functions_Funs_Included. eassumption.
           apply Union_Disjoint_l. now eauto with Ensembles_DB.
-          eapply Disjoint_Included_l_sym; [| eassumption ].
+          eapply Disjoint_Included_l_sym. 
           now apply name_in_fundefs_bound_var_fundefs.
+          eapply Union_Disjoint_l; eauto.
+          eapply Disjoint_Included; [| | now apply Hf ]...
         * eapply Disjoint_Included_l.
           eapply Add_functions_FunsFVs_Included_r. eassumption.
           apply Union_Disjoint_l. now eauto with Ensembles_DB.
           eapply Disjoint_Included_l. eassumption.
-          eapply Union_Disjoint_l.
-          eapply Disjoint_sym. eapply Disjoint_Included; [ | | now apply HD ].
-          normalize_occurs_free...  now eauto with Ensembles_DB.
-          eapply Disjoint_Included_r; [| eassumption ]...
+          eapply Union_Disjoint_r. eapply Union_Disjoint_l.
+          eapply Disjoint_sym. eapply Disjoint_Included; [ | | now apply Hf ].
+          normalize_occurs_free...  eassumption.
+          eapply Union_Disjoint_l...
+          eapply Union_Disjoint_l. eapply Disjoint_sym.
+          eapply Disjoint_Included; [ | | now apply HD ].
+          normalize_occurs_free... now eauto with Ensembles_DB.
+          eapply Union_Disjoint_l...
         * eapply Disjoint_Included_r.
           now eapply occurs_free_Efun_Included.
           apply Union_Disjoint_r. now eauto with Ensembles_DB.
@@ -1589,21 +2144,29 @@ Section Lambda_lifting_correct.
           eassumption. 
         * eapply binding_in_map_antimon;
           [| eapply binding_in_map_def_funs; eassumption ].
-          apply Union_Included. rewrite Union_assoc.
-          apply Included_Union_preserv_l. normalize_occurs_free. 
-          rewrite Union_assoc, Union_Setminus_Included;
-            now eauto with Ensembles_DB typeclass_instances.
-          eapply Included_trans.
-          eapply Add_functions_FunsFVs_Included_r. eassumption.
-          eapply Union_Included. now eauto with Ensembles_DB.
-          eapply Included_trans. eassumption.
-          normalize_occurs_free...
+          eapply Included_trans. eapply Add_functions_image_Included. eassumption.
+          rewrite (Union_commut (name_in_fundefs B')).
+          eapply Included_Union_compat.
+          eapply image_monotonic. rewrite !Setminus_Union_distr.
+          eapply Union_Included. eapply Union_Included.
+          rewrite <- Setminus_Union. normalize_occurs_free...
+          eapply Included_trans. eapply Included_Setminus_compat.
+          eapply Add_functions_FunsFVs_Included_r; eauto. reflexivity.
+          rewrite !Setminus_Union_distr. eapply Union_Included.
+          now eauto with Ensembles_DB. eapply Setminus_Included_Included_Union.
+          eapply Included_trans. eassumption. normalize_occurs_free.
+          now eauto 15 with Ensembles_DB. 
+          eapply Included_trans. eapply Included_Setminus_compat.
+          eapply Add_functions_LiftedFuns_Included_r; eauto. reflexivity.
+          rewrite !Setminus_Union_distr, (Setminus_Included_Empty_set (Setminus var S S'0)).
+          rewrite Union_Empty_set_neut_r...
+          now eauto with Ensembles_DB.
+          rewrite Add_functions_Fundefs_lambda_lift_name_in_fundefs with (B2 := B'); eauto.
+          now eauto with Ensembles_DB. reflexivity.
         * eapply preord_env_P_inj_antimon. eassumption.
-          apply Union_Included.
-          apply Included_Union_preserv_l. normalize_occurs_free. 
+          normalize_occurs_free. 
           rewrite Union_commut, Union_assoc, Union_Setminus_Included;
             now eauto with Ensembles_DB typeclass_instances.
-          now eauto with Ensembles_DB.
     - intros v1 c1 Hleq Hstep. inv Hstep.
       edestruct preord_env_P_inj_getlist_l as [vs' [Hgetl' Hprevs]]; try eassumption.
       normalize_occurs_free...
@@ -1620,7 +2183,7 @@ Section Lambda_lifting_correct.
       eassumption. now eauto. eassumption.
       eapply preord_val_monotonic. eassumption. omega.
     - eapply preord_exp_app_compat.
-      eapply Henv. now left; eauto.
+      now eapply Henv.
       eapply Forall2_preord_var_env_map. eassumption.
       normalize_occurs_free...
     - inv Hun. eapply preord_exp_prim_compat.
@@ -1632,11 +2195,10 @@ Section Lambda_lifting_correct.
           rewrite occurs_free_Eprim in Him.
           eapply Disjoint_Included; [ | | now apply Him ].
           normalize_bound_var...
-          apply image_monotonic. rewrite Setminus_Union_distr...
+          apply image_monotonic. rewrite !Setminus_Union_distr...
           eapply Union_Disjoint_r.
           eapply Disjoint_Included_l_sym; [| eassumption ]...
-          eapply Disjoint_Singleton_l. intros Hc. inv Hc. now eauto.
-          eapply Hlf. now constructor; eauto.
+          now eapply Disjoint_Singleton_l.
         * eapply Disjoint_Included_r; [| eassumption ].
           now apply bound_var_occurs_free_Eprim_Included.
         * repeat normalize_bound_var_in_ctx...
@@ -1647,19 +2209,17 @@ Section Lambda_lifting_correct.
           eapply Disjoint_Included_l ; [| now apply HD].
           normalize_bound_var... now apply Disjoint_Singleton_r.
         * eapply binding_in_map_antimon; [| eapply binding_in_map_set; eassumption ]. 
-          apply Union_Included; [| now eauto with Ensembles_DB ].
-          rewrite Union_commut, Union_assoc.
-          apply Included_Union_preserv_l.
-          normalize_occurs_free. rewrite Union_assoc.
-          rewrite Union_Setminus_Included;
-            now eauto with Ensembles_DB typeclass_instances.
+          eapply Included_trans. eapply image_extend_Included'.
+          eapply Included_Union_compat; [| reflexivity ].
+          eapply image_monotonic. rewrite !Setminus_Union_distr.
+          normalize_occurs_free...
         * eapply preord_env_P_inj_set_alt. 
           eapply preord_env_P_inj_antimon. eassumption.
-          rewrite Setminus_Union_distr; normalize_occurs_free...
+          normalize_occurs_free...
           eassumption.
           intros Hc. eapply Him. constructor; eauto.
           eapply image_monotonic; [| eassumption ].
-          rewrite Setminus_Union_distr; normalize_occurs_free...
+          normalize_occurs_free...
         * eapply Funs_inv_set.
           intros Hc. eapply Hfun. now constructor; eauto.
           intros Hc. eapply Hlf. now constructor; eauto.
@@ -1668,7 +2228,7 @@ Section Lambda_lifting_correct.
           eapply image_monotonic; [| eassumption ]...
           eassumption.
     - eapply preord_exp_halt_compat.
-      eapply Henv; left; eauto.
+      eapply Henv; eauto.
   Qed.
 
 End Lambda_lifting_correct.
